Working on finalization tactics.

examples/QueryStructure/BookstorewDelegationSemiAutomatic.v
@@ -288,6 +288,43 @@ Ltac implement_Pick_DelegateToBag_AbsR_observer :=
       => setoid_rewrite (refine_pick_val (@DelegateToBag_AbsR qs_schema indices r_o) H)
   end.
 
+  Add Parametric Morphism
+      (A : Type)
+      (f : A -> Type)
+      (As : list A)
+      (a : A)
+      (l' : list (ilist f As))
+      : (@Join_Lists A f As a l')
+      with signature
+      (pointwise_relation _ refine) ==> refine
+        as refine_Join_Lists.
+  Proof.
+    unfold pointwise_relation; simpl; intros.
+    induction l'; unfold Join_Lists; simpl.
+    - reflexivity.
+    - rewrite H; setoid_rewrite IHl'; reflexivity.
+  Qed.
+
+Lemma refine_Join_Enumerate_Swap
+      qs_schema BagIndexKeys
+        (ResultT : Type) :
+    forall r_o (r_n : IndexedQueryStructure qs_schema BagIndexKeys),
+      DelegateToBag_AbsR r_o r_n ->
+      forall (idx idx' : BoundedString)
+             (resultComp : _ -> Comp (list ResultT)),
+        refine (l <- CallBagMethod idx {|bindex := "Enumerate" |} r_n ();
+                l' <- (Join_Lists (Build_single_Tuple_list (snd l))
+                                  (fun _ => l <- (CallBagMethod idx' {|bindex := "Enumerate" |} r_n ());
+                                   ret (snd l)));
+                List_Query_In l' resultComp)
+               (l <- CallBagMethod idx' {|bindex := "Enumerate" |} r_n ();
+                l' <- (Join_Lists (Build_single_Tuple_list (snd l))
+                                  (fun _ => l <- (CallBagMethod idx {|bindex := "Enumerate" |} r_n ());
+                                   ret (snd l)));
+                List_Query_In l' (fun tup_pair => (resultComp (icons _ (ilist_hd (ilist_tl tup_pair)) (icons _ (ilist_hd tup_pair) (inil _)))))).
+  Proof.
+  Admitted.
+
 (* implement_In' implements [UnConstrQuery_In] in a variety of contexts. *)
 Ltac implement_In' :=
   match goal with
@@ -296,7 +333,7 @@ Ltac implement_In' :=
     | [H : @DelegateToBag_AbsR ?qs_schema ?indexes ?r_o ?r_n
        |- context[fun b' : ?ElementT => List_Query_In (@?l b') (fun b => UnConstrQuery_In (ResultT := ?resultT) ?r_o ?idx (@?f b' b) )] ] =>
       let H' := eval simpl in
-      (fun (b' : ElementT) => refine_Join_Query_In_Enumerate' H (idx := idx) (f b') (l b')) in
+      (fun (b' : ElementT) => refine_Join_Query_In_Enumerate' H idx (f b') (l b')) in
           setoid_rewrite H'
 
     (* Implement a 'naked' UnConstrQuery_In as a call to enumerate *)
@@ -313,30 +350,13 @@ Ltac implement_In' :=
           setoid_rewrite H'
   end.
 
-Ltac implement_In :=    
+Ltac implement_In :=
   (* First simplify any large terms [i.e. Rep, BagSpec, snd, and MethodDomCod
      that might slow down setoid rewriting *)
   simpl in *;
   (* The repeatedly implement [In]s *)
   repeat implement_In'.
 
-Theorem BookStoreManual :
-  Sharpened BookStoreSpec.
-Proof.
-
-  unfold BookStoreSpec.
-
-  (* First, we unfold various definitions and drop constraints *)
-  start honing QueryStructure.
-
-  make simple indexes using [[sAUTHOR; sISBN]; [sISBN]].
-
-  hone constructor "Init".
-  {
-    simplify with monad laws.
-    rewrite refine_QSEmptySpec_Initialize_IndexedQueryStructure.
-    finish honing.
-  }
 
   Fixpoint Join_ListsT (Ts : list Type) : Type
     :=
@@ -345,128 +365,63 @@ Proof.
         | [A] => A
         | A :: Cs => prod A (Join_ListsT Cs)
       end.
-  
-  Inductive list' (A : Type) : Type :=
-  | nil' : list' A | cons' : A -> list' A -> list' A.
 
-  Fixpoint list'_to_list
-           (A : Type)
-           (l : list' A)
-  : list A :=
-    match l with
-      | nil' => nil
-      | cons' a As => cons a (list'_to_list As)
-    end.
-
-  Fixpoint list_to_list'
-           (A : Type)
-           (l : list A)
-  : list' A :=
-    match l with
-      | nil => nil' A
-      | cons a As => cons' a (list_to_list' As)
-    end.
-
-  Lemma list_to_list'_id {A : Type}
-  : forall l : list' A,
-      list_to_list' (list'_to_list l) = l.
+  Lemma ExtensionalEq_andb {A} :
+    forall (f g f' g' : A -> bool),
+      ExtensionalEq f f'
+      -> ExtensionalEq g g'
+      -> ExtensionalEq (fun a => f a && g a) (fun a => f' a && g' a).
   Proof.
-    induction l; simpl; congruence.
+    unfold ExtensionalEq; intros; congruence.
   Qed.
 
-  Lemma list'_to_list_id {A : Type}
-  : forall l : list A,
-      list'_to_list (list_to_list' l) = l.
+  Lemma ExtensionalEq_andb_true {A} :
+    forall (f f' : A -> bool),
+      ExtensionalEq f f'
+      -> ExtensionalEq f (fun a => f' a && (fun _ => true) a).
   Proof.
-    induction l; simpl; congruence.
+    unfold ExtensionalEq; intros.
+    rewrite andb_true_r; apply H.
   Qed.
 
-  (* Fixpoint Join_Lists''
-           {A : Type}
-           (Ts : list A)
-           (f : A -> Type)
-           (ls : ilist (fun a => list' (f a))  Ts)
-  : @list (ilist f Ts). *)
-
-  Lemma refineEquiv_Join_bind {A B C}
-  : let T := Type in
-    forall (ca : Comp A)
-           (cb : Comp B)
-           (c : A -> B -> Comp C),
-      refine (a <- ca;
-              b <- cb;
-              c a b)
-             (ab <- (a <- ca;
-                     b <- cb;
-                     ret (icons (A := T) (B := id) A a (icons (A := T) (B := id) B b (inil id))));
-              c (ith_default (A := T) (B := id) unit () ab 0)
-                (ith_default (A := T) (B := id) unit () ab 1)).
-  Proof.
-    intros * v Comp_v; inversion_by computes_to_inv; subst;
-    repeat econstructor; eauto.
-  Qed.
-
-  (*Lemma refineEquiv_Join_bind' {A B C} {D D'}
-  : forall (ca : Comp (D * (list A)))
-           (cb : Comp (D' * (list B)))
-           (c : list (A * B) -> Comp C),
-      refine (a <- ca;
-              b <- cb;
-              c (Join_Lists (snd a) (Build_single_Tuple_list (snd b))))
-             (ab <- (a <- ca;
-                     b <- cb;
-                     ret (icons A (list_to_list' (snd a)) (icons B (list_to_list' (snd b)) (inil list'))));
-              c (Join_Lists'' ab)).
-  Proof.
-    intros; rewrite refineEquiv_Join_bind.
-    simpl; intros v Comp_v; inversion_by computes_to_inv; subst.
-    repeat econstructor; eauto.
-    simpl in *; repeat rewrite list'_to_list_id in H1; eauto.
-  Qed. *)
-  
-  hone method "NumOrders".
-  {
-    simplify with monad laws.
-    implement_In.
-    simpl; repeat (setoid_rewrite refine_List_Query_In_Where;
-                   instantiate (1 := _)); simpl; 
-    repeat setoid_rewrite <- filter_and.
+  Ltac split_filters k :=
     match goal with
-        |- context[filter ?f _] =>
-        let T := type of f in 
+      | |- ExtensionalEq (fun a => (@?f a) && (@?g a)) ?b =>
+        let fT := type of f in
+        let gT := type of g in
+        makeEvar
+          fT
+          ltac:(fun f' =>
+                  makeEvar gT ltac:(fun g' =>
+                                      apply (@ExtensionalEq_andb _ f g f' g');
+                                    [ first [split_filters | k ] | first [split_filters | k]] ))
+      | |- ExtensionalEq (fun a => (@?f a)) ?b =>
+        let fT := type of f in
+        makeEvar
+          fT
+          ltac:(fun f' => k)
+    end.
+
+  (* Convert List_Query_In Where Clauses into a filter using search terms. *)
+  Ltac convert_Where_to_search_term :=
+    (* First replace Where clauses with test functions. *)
+    simpl; repeat (setoid_rewrite refine_List_Query_In_Where;
+                   instantiate (1 := _)); simpl;
+    (* Combine different filters into a single function. *)
+    repeat setoid_rewrite <- filter_and;
+    (* Now break the functions up again and find search term replacements for each. *)
+    match goal with
+        |- context [List_Query_In (filter ?f _) _] =>
+        let T := type of f in
         makeEvar T
                  ltac:(fun g =>
-                         let eqv := fresh in 
+                         let eqv := fresh in
                          assert (ExtensionalEq f g) as eqv;
-                       [
+                       [ apply ExtensionalEq_andb_true; split_filters idtac
                        | setoid_rewrite (filter_by_equiv f g eqv)])
     end.
 
-    Lemma ExtensionalEq_andb {A} :
-      forall (f g f' g' : A -> bool),
-        ExtensionalEq f f'
-        -> ExtensionalEq g g'
-        -> ExtensionalEq (fun a => f a && g a) (fun a => f' a && g' a).
-    Proof.
-      unfold ExtensionalEq; intros; congruence.
-    Qed.
-
-    Ltac split_filters k :=
-      match goal with
-          |- ExtensionalEq (fun a => (@?f a) && (@?g a)) ?b =>
-          let fT := type of f in
-          let gT := type of g in
-          makeEvar
-            fT
-            ltac:(fun f' =>
-                    makeEvar gT ltac:(fun g' =>
-                                        apply (@ExtensionalEq_andb _ f g f' g');
-                                      [ first [split_filters | k ] | first [split_filters | k]] ))
-    end.
-
-    split_filters idtac.
-
-    Ltac equate X Y := let H := fresh in assert (H : X = Y) by reflexivity; clear H.
+  Ltac equate X Y := let H := fresh in assert (H : X = Y) by reflexivity; clear H.
 
     Definition unit_Heading :=
       {| Attributes := unit;
@@ -474,7 +429,7 @@ Proof.
 
     Definition unit_Tuple : @Tuple unit_Heading := id.
 
-    Ltac get_ithDefault f n k := 
+    Ltac get_ithDefault f n k :=
       match type of f with
         | ilist (@Tuple) ?A -> ?C =>
           let G := fresh "G" in
@@ -495,9 +450,7 @@ Proof.
         let G' := eval unfold G in G in clear G; k G'
       end.
 
-    Focus 2.
-
-    Ltac get_ithDefault_pair f m n k := 
+    Ltac get_ithDefault_pair f m n k :=
       match type of f with
         | ilist (@Tuple) ?A -> ?C =>
           let G := fresh "G" in
@@ -506,21 +459,21 @@ Proof.
           let proj1 := fresh "proj" in
           let proj2 := fresh "proj" in
           let proj1 := eval simpl in
-          (fun b : ilist (@Tuple) A => ith_default unit_Heading unit_Tuple b m) in 
+          (fun b : ilist (@Tuple) A => ith_default unit_Heading unit_Tuple b m) in
           let proj2 := eval simpl in
           (fun b : ilist (@Tuple) A => ith_default unit_Heading unit_Tuple b n)
             in evar (G : @Tuple (nth_default unit_Heading A m)
                          -> @Tuple (nth_default unit_Heading A n)
                          -> C);
              assert (H : forall p,
-                           f p = G (proj1 p) (proj2 p)) by 
+                           f p = G (proj1 p) (proj2 p)) by
               ( subst G; intro p;
                let p1 := eval simpl in (proj1 p) in
-               let p2 := eval simpl in (proj2 p) in 
+               let p2 := eval simpl in (proj2 p) in
                pattern p1, p2;
                  match goal with
                    | [ |- (fun t t' => @?f t t' = @?g t t') _ _ ] => equate f g; reflexivity
-                 end); clear H; 
+                 end); clear H;
              let G' := eval unfold G in G in clear G; k G'
       end.
 
@@ -562,6 +515,10 @@ Ltac makeTerm_dep dom fs SC fds tail k :=
     createTerm_dep dom fs f fds tail k
   end.
 
+Definition Dep_SearchTerm_Wrapper {A} {heading}
+           (search_term_dep : @Tuple heading -> A)
+           (tup : @Tuple heading) : A := search_term_dep tup.
+
 Ltac find_simple_search_term_dep qs_schema idx dom filter_dec search_term :=
   match type of search_term with
     | ?dom -> BuildIndexSearchTerm ?attr =>
@@ -571,8 +528,9 @@ Ltac find_simple_search_term_dep qs_schema idx dom filter_dec search_term :=
                                let tail := eval simpl in tail in
                                    makeTerm_dep dom attr SC fds tail
                                                 ltac:(fun tm => pose tm;
-                                                      (* unification fails if I don't pose tm first... *) unify tm search_term;
-                                                      unfold ExtensionalEq, MatchIndexSearchTerm; 
+                                                      (* unification fails if I don't pose tm first... *)
+                                                      unify (Dep_SearchTerm_Wrapper tm) search_term;
+                                                      unfold ExtensionalEq, MatchIndexSearchTerm;
                                                       simpl; intros;
                                                       try prove_extensional_eq))
   end.
@@ -590,7 +548,7 @@ Ltac find_equivalent_tuple schemas heading k :=
         || find_equivalent_tuple schemas' heading k
   end.
 
-Ltac find_equivalent_search_term_pair m n build_search_term_dep := 
+Ltac find_equivalent_search_term_pair m n build_search_term_dep :=
 match goal with
     [ H : @DelegateToBag_AbsR ?qs_schema ?indices ?r_o ?r_n
       |- ExtensionalEq ?f _ ] =>
@@ -602,14 +560,14 @@ match goal with
         let heading := match type of filter_dec with
                          | ?A -> @Tuple ?heading -> bool => constr:(heading)
                        end in
-        let schemas := eval simpl in (qschemaSchemas qs_schema) in 
-            find_equivalent_tuple schemas heading 
+        let schemas := eval simpl in (qschemaSchemas qs_schema) in
+            find_equivalent_tuple schemas heading
               ltac:(fun id => let idx' := constr:({| bindex := id |} : BoundedIndex (map relName (qschemaSchemas qs_schema)))
                               in let idx := eval simpl in idx' in
     let idx_search_update_term := eval simpl in (ith_Bounded relName indices idx) in
     let search_term_type := eval simpl in (BagSearchTermType idx_search_update_term) in
         let search_term_matcher := eval simpl in (BagMatchSearchTerm idx_search_update_term) in
-        makeEvar (dom -> search_term_type) 
+        makeEvar (dom -> search_term_type)
                  ltac: (fun search_term =>
                           let eqv := fresh in
                           assert (forall a b, filter_dec a b
@@ -619,7 +577,7 @@ match goal with
                         | match goal with
                             |- ExtensionalEq ?f ?search_term' =>
                             match type of f with
-                                | ?A -> _ => 
+                                | ?A -> _ =>
                                   unify search_term' (fun a : A => search_term_matcher (search_term (ith_default unit_Heading unit_Tuple a m))
             ((ith_default unit_Heading unit_Tuple a n)))
                             end
@@ -628,26 +586,23 @@ match goal with
                           simpl in *; rewrite eqv; reflexivity
 ]))) end.
 
-Unset Ltac Debug.
-find_equivalent_search_term_pair 0 1 find_simple_search_term_dep.
-
-Ltac find_equivalent_search_term m build_search_term := 
+Ltac find_equivalent_search_term m build_search_term :=
 match goal with
     [ H : @DelegateToBag_AbsR ?qs_schema ?indices ?r_o ?r_n
       |- ExtensionalEq ?f _ ] =>
-    get_ithDefault f m 
+    get_ithDefault f m
       ltac:(fun filter_dec =>
         let heading := match type of filter_dec with
                          | @Tuple ?heading -> bool => constr:(heading)
                        end in
-        let schemas := eval simpl in (qschemaSchemas qs_schema) in 
-            find_equivalent_tuple schemas heading 
+        let schemas := eval simpl in (qschemaSchemas qs_schema) in
+            find_equivalent_tuple schemas heading
               ltac:(fun id => let idx' := constr:({| bindex := id |} : BoundedIndex (map relName (qschemaSchemas qs_schema)))
                               in let idx := eval simpl in idx' in
     let idx_search_update_term := eval simpl in (ith_Bounded relName indices idx) in
     let search_term_type := eval simpl in (BagSearchTermType idx_search_update_term) in
         let search_term_matcher := eval simpl in (BagMatchSearchTerm idx_search_update_term) in
-        makeEvar (search_term_type) 
+        makeEvar (search_term_type)
                  ltac: (fun search_term =>
                           let eqv := fresh in
                           assert (forall a, filter_dec a
@@ -657,7 +612,7 @@ match goal with
                         | match goal with
                               |- ExtensionalEq ?f ?search_term' =>
                               match type of f with
-                                | ?A -> _ => 
+                                | ?A -> _ =>
                                   unify search_term' (fun a : A => search_term_matcher search_term (ith_default unit_Heading unit_Tuple a m))
                               end
                           end;
@@ -665,13 +620,143 @@ match goal with
                           simpl in *; rewrite eqv; reflexivity
 ]))) end.
 
-find_equivalent_search_term 0 find_simple_search_term.
-simpl
-Focus 3.
-match goal with
-    |- ExtensionalEq ?f ?b =>
-    get_ithDefault f 0 ltac:(fun l => pose l)
-end.
+Corollary refine_Join_Lists_filter_filter_search_term_snd_dep'
+          qs_schema BagIndexKeys
+        (ResultT : Type) :
+    forall (r_n : IndexedQueryStructure qs_schema BagIndexKeys)
+           idx idx'
+           (search_pattern : _ -> _)
+           (resultComp : ilist (@Tuple) [_; _] -> Comp (list ResultT))
+           filter_rest st,
+      refine (cl <- CallBagMethod idx {| bindex := "Find" |} r_n st;
+              l' <- (Join_Lists (Build_single_Tuple_list (snd cl))
+                                (fun _ => l <- CallBagMethod idx' {| bindex := "Enumerate" |} r_n ();
+                                 ret (snd l)));
+              List_Query_In (filter (fun a : ilist (@Tuple) [_ ; _] => BagMatchSearchTerm _ (search_pattern (ilist_tl a)) (ilist_hd a) && filter_rest a) l')
+                            resultComp)
+             (cl <- CallBagMethod idx {| bindex := "Find" |} r_n st;
+              l' <- (Join_Lists (Build_single_Tuple_list (snd cl))
+                                (fun tup => l <- CallBagMethod idx' {| bindex := "Find" |} r_n (search_pattern tup);
+                                             ret (snd l)));
+                      List_Query_In (filter filter_rest l') resultComp).
+  Proof.
+    intros; f_equiv; intro;
+    apply refine_Join_Lists_filter_search_term_snd_dep.
+  Qed.
+
+  Ltac convert_filter_to_find':=
+    try match goal with
+            |- context[filter (fun a => (_ && _) && true) _] =>
+            setoid_rewrite <- andb_assoc; simpl
+        end;
+    match goal with
+      | H : @DelegateToBag_AbsR ?qs_schema ?indices ?r_o ?r_n
+        |- context[l <- CallBagMethod ?idx ``("Enumerate") ?r_n ();
+                    List_Query_In (filter (fun a => MatchIndexSearchTerm ?st (ilist_hd a) && @?filter_rest a)
+                                          (Build_single_Tuple_list (snd l))) ?resultComp] =>
+        let b := fresh in
+        pose proof (@refine_Query_For_In_Find_single _ _ _ r_o r_n H idx st resultComp filter_rest) as b;
+          simpl in b; setoid_rewrite b; clear b
+
+      | H : @DelegateToBag_AbsR ?qs_schema ?indices ?r_o ?r_n
+        |- context[l <- CallBagMethod ?idx ``("Enumerate") ?r_n ();
+                    l' <- Join_Lists (Build_single_Tuple_list (snd l)) ?cl;
+                    List_Query_In (filter (fun a => MatchIndexSearchTerm ?st (ilist_hd (ilist_tl a)) && @?filter_rest a)
+                                          l') ?resultComp] =>
+        let b := fresh in
+        pose proof (fun foo => @refine_Join_Lists_filter_search_term_fst _ _ _ r_n idx _ cl st resultComp foo filter_rest) as b;
+          simpl in b; setoid_rewrite b;
+          [ clear b
+          | match goal with
+              | |- context [CallBagMethod ?idx' ``("Enumerate") _ _] =>
+                intros; eapply (realizeable_Enumerate (r_o := r_o) (r_n := r_n) idx' H)
+              | |- context [CallBagMethod ?idx' ``("Find") _ _] =>
+                intros; eapply (realizeable_Find (r_o := r_o) (r_n := r_n) idx' H)
+            end]
+      | H : @DelegateToBag_AbsR ?qs_schema ?indices ?r_o ?r_n
+        |- context[l <- CallBagMethod ?idx ``("Find") ?r_n ?st;
+                    l' <- Join_Lists (Build_single_Tuple_list (snd l))
+                       (fun _ : ilist (@Tuple) [?heading] =>
+                          l <- CallBagMethod ?idx' ``("Enumerate") ?r_n ();
+                        ret (snd l));
+                    List_Query_In (filter (fun a => MatchIndexSearchTerm (Dep_SearchTerm_Wrapper ?st' (ilist_hd (ilist_tl a)))
+                                                                         (ilist_hd a) && @?filter_rest a) l') ?resultComp] =>
+        let b := fresh in
+        pose proof (@refine_Join_Lists_filter_filter_search_term_snd_dep' _ _ _ r_n idx idx'
+                                                                          (fun a => Dep_SearchTerm_Wrapper st' (ilist_hd a))
+                                                                          resultComp filter_rest st) as b;
+          unfold Dep_SearchTerm_Wrapper in b; simpl in b; setoid_rewrite b; clear b
+      (* The final case replaces the last filter and the Return statement. *)
+      | _ => setoid_rewrite filter_true; setoid_rewrite refine_List_Query_In_Return
+    end.
+
+  Ltac convert_filter_to_find :=
+    simpl; repeat convert_filter_to_find'.
+
+  (* This also implements Fors *)
+  Ltac Implement_Aggregates :=
+    repeat
+      match goal with
+        | |- context[For _] => setoid_rewrite refine_For_List
+        | |- context[Count _] => setoid_rewrite refine_Count
+      end.
+
+  (* Commits the database at the end of a method call. *)
+  Ltac commit :=
+    match goal with
+      | [H : @DelegateToBag_AbsR ?qs_schema ?indices ?r_o ?r_n
+         |- context[{r_n' : IndexedQueryStructure ?qs_schema ?indices | DelegateToBag_AbsR ?r_o r_n'}] ]
+        => setoid_rewrite (refine_pick_val (@DelegateToBag_AbsR qs_schema indices r_o) H);
+          simplify with monad laws
+    end.
+
+Theorem BookStoreManual :
+  Sharpened BookStoreSpec.
+Proof.
+
+  unfold BookStoreSpec.
+
+  (* First, we unfold various definitions and drop constraints *)
+  start honing QueryStructure.
+
+  make simple indexes using [[sAUTHOR; sISBN]; [sISBN]].
+
+  hone constructor "Init".
+  {
+    simplify with monad laws.
+    rewrite refine_QSEmptySpec_Initialize_IndexedQueryStructure.
+    finish honing.
+  }
+
+  hone method "NumOrders".
+  {
+    simplify with monad laws.
+    implement_In.
+    setoid_rewrite refine_Join_Enumerate_Swap; eauto.
+    convert_Where_to_search_term.
+
+    find_equivalent_search_term 1 find_simple_search_term.
+    find_equivalent_search_term_pair 1 0 find_simple_search_term_dep.
+
+    convert_filter_to_find.
+    Implement_Aggregates.
+    commit.
+    finish honing.
+  }
+
+  hone method "GetTitles".
+  {
+    simplify with monad laws.
+    implement_In.
+    convert_Where_to_search_term.
+
+    find_equivalent_search_term 0 find_simple_search_term.
+
+    convert_filter_to_find.
+    Implement_Aggregates.
+    commit.
+    finish honing.
+}
 
   hone method "DeleteOrder".
   {
@@ -682,36 +767,6 @@ end.
     finish honing.
   }
 
-
-
-    setoid_rewrite r.
-    setoid_rewrite refine_Join_Query_In_Enumerate'.
-    refine_List_Query_In_Where.
-    implement_Enumerate_filter find_simple_search_term.
-    simplify with monad laws.
-    simpl; implement_Pick_DelegateToBag_AbsR_observer; simplify with monad laws.
-    setoid_rewrite refine_List_Query_In_Return.
-    simplify with monad laws.
-    finish honing.
-  }
-
-  hone method "GetTitles".
-  {
-    setoid_rewrite refine_Query_In_Enumerate; eauto.
-    setoid_rewrite refine_List_Query_In_Where.
-    implement_Enumerate_filter find_simple_search_term.
-    simplify with monad laws.
-    simpl; implement_Pick_DelegateToBag_AbsR_observer; simplify with monad laws.
-    setoid_rewrite refine_List_Query_In_Return.
-    simplify with monad laws.
-    finish honing.
-  }
-
-  hone method "NumOrders".
-  {
-
-  unfold cast, eq_rect_r, eq_rect, eq_sym; simpl.
-
   (* At this point our implementation is fully computational: we're done! *)
 
   Require Import ADTNotation.BuildComputationalADT.
@@ -719,26 +774,872 @@ end.
 
   Ltac FullySharpenEachMethod delegateSigs delegateSpecs cRep' cAbsR' :=
     match goal with
-        |- Sharpened (@BuildADT ?Rep ?consSigs ?methSigs ?consDefs ?methDefs) =>
-        ilist_of_evar
-          (ilist ComputationalADT.cADT delegateSigs)
-          (fun DelegateImpl Sig => cMethodType (cRep' DelegateImpl) (methDom Sig) (methCod Sig))
-          methSigs
-          ltac:(fun cMeths => ilist_of_evar
-                                (ilist ComputationalADT.cADT delegateSigs)
-                                (fun DelegateImpl Sig =>
-                                   cConstructorType (cRep' DelegateImpl) (consDom Sig))
-                                consSigs
-                                ltac:(fun cCons =>
-                                        eapply Notation_Friendly_SharpenFully with
-                                        (DelegateSpecs := delegateSpecs)
-                                          (cConstructors := cCons)
-                                          (cMethods := cMeths)
-                                          (cAbsR := cAbsR')));
-          unfold Dep_Type_BoundedIndex_app_comm_cons
-    end.
+      |- Sharpened (@BuildADT ?Rep ?consSigs ?methSigs ?consDefs ?methDefs) => 
+      ilist_of_evar
+        (ilist (fun nadt => ComputationalADT.cADT (namedADTSig nadt)) delegateSigs)
+        (fun DelegateImpl Sig => ComputationalADT.cMethodType (cRep' DelegateImpl) (methDom Sig) (methCod Sig))
+        methSigs
+        ltac:(fun cMeths => 
+                ilist_of_evar
+                  (ilist (fun nadt => ComputationalADT.cADT (namedADTSig nadt)) delegateSigs)
+                  (fun DelegateImpl Sig => ComputationalADT.cConstructorType (cRep' DelegateImpl) (consDom Sig))
+                  consSigs
+                  ltac:(fun cCons =>  
+                          eapply
+                            (@Notation_Friendly_SharpenFully
+                               _ 
+                               consSigs
+                               methSigs
+                               consDefs
+                               methDefs
+                               delegateSigs
+                               cRep'
+                               cCons
+                               cMeths
+                               delegateSpecs
+                               cAbsR')));
+        unfold Dep_Type_BoundedIndex_app_comm_cons
+    end; simpl; split.
 
-  FullySharpenEachMethod [BagSig Book (BuildSearchTermFromAttributes BookSearchTerm);
+  Fixpoint Build_IndexedQueryStructure_Impl_Sigs
+    {indices : list NamedSchema}
+      (Index : ilist (fun ns : NamedSchema => SearchUpdateTerms (schemaHeading (relSchema ns))) indices)
+    : list NamedADTSig :=
+    match indices as indices return ilist _ indices -> list NamedADTSig with
+      | nil => fun _ => nil
+      | cons ns indices' =>
+        fun Index =>
+          {| ADTSigname := relName ns;
+             namedADTSig := 
+               BagSig (@Tuple (schemaHeading (relSchema ns))) (BagSearchTermType (ilist_hd Index)) (BagUpdateTermType (ilist_hd Index)) |}
+                       :: @Build_IndexedQueryStructure_Impl_Sigs indices' (ilist_tl Index)
+    end Index.
+
+  Fixpoint Build_IndexedQueryStructure_Impl_Specs
+           {indices : list NamedSchema}
+           (Index : ilist (fun ns : NamedSchema => SearchUpdateTerms (schemaHeading (relSchema ns))) indices)
+  : ilist (fun ns => ADT (namedADTSig ns)) (@Build_IndexedQueryStructure_Impl_Sigs indices Index) :=
+    match indices as indices return
+          forall (Index : ilist _ indices),
+            ilist (fun ns : NamedADTSig => ADT (namedADTSig ns))
+                  (@Build_IndexedQueryStructure_Impl_Sigs indices Index)
+    with
+      | nil => fun _ => inil _
+      | cons ns indices' =>
+        fun Index => icons {| ADTSigname := relName ns;
+                              namedADTSig := _ |}
+                           (@BagSpec (@Tuple (schemaHeading (relSchema ns)))
+                                     (BagSearchTermType (ilist_hd Index))
+                                     (BagUpdateTermType (ilist_hd Index))
+                                     (BagMatchSearchTerm (ilist_hd Index))
+                                     (BagApplyUpdateTerm (ilist_hd Index)))
+                           (@Build_IndexedQueryStructure_Impl_Specs indices' (ilist_tl Index))
+    end Index.
+  
+  Definition Build_IndexedQueryStructure_Impl_cRep
+           {indices : list NamedSchema}
+           (Index : ilist (fun ns : NamedSchema => SearchUpdateTerms (schemaHeading (relSchema ns))) indices)
+           (DelegateImpls : ilist (fun ns => cADT (namedADTSig ns)) (@Build_IndexedQueryStructure_Impl_Sigs indices Index))
+  : Type
+    :=
+    i2list
+      (fun (ns : NamedADTSig)
+           (index : cADT (namedADTSig ns)) => cRep index) DelegateImpls.
+
+  Fixpoint map_IndexedQS_idx_boundi
+        {indices}
+  : forall
+      n
+      (Index : ilist
+                 (fun ns : NamedSchema =>
+                    SearchUpdateTerms (schemaHeading (relSchema ns)))
+                 indices)
+      idx, 
+      nth_error
+        (map ADTSigname (Build_IndexedQueryStructure_Impl_Sigs Index))
+        n = Some idx
+      ->  nth_error (map relName indices) n = Some idx.
+  Proof.
+    refine (match indices with
+              | nil => _
+              | ns :: indices' =>
+                fun n => 
+                  match n return
+                        forall
+                          (Index : ilist
+                                     (fun ns : NamedSchema =>
+                                        SearchUpdateTerms (schemaHeading (relSchema ns)))
+                                     (ns :: indices'))
+                          idx,
+                          nth_error (map ADTSigname (Build_IndexedQueryStructure_Impl_Sigs Index)) n =
+                          Some idx ->
+                          nth_error (map relName (ns :: indices')) n = Some idx
+                  with
+                    | 0 => fun Index idx nth_n => nth_n
+                    | S n' => fun Index => (map_IndexedQS_idx_boundi indices' n' (ilist_tl Index))
+                  end
+            end);
+    simpl; intros; try discriminate; eauto.
+  Defined.
+  
+  Definition map_IndexedQS_idx
+             indices
+             (Index : ilist (fun ns : NamedSchema => SearchUpdateTerms (schemaHeading (relSchema ns))) indices )
+             (idx : BoundedIndex
+                      (map ADTSigname
+                           (Build_IndexedQueryStructure_Impl_Sigs Index)))
+  : BoundedIndex (map relName indices) := 
+    {| bindex := bindex idx;
+       indexb := {| ibound := ibound (indexb idx);
+                    boundi := map_IndexedQS_idx_boundi _ Index (boundi (indexb idx))|} |}.
+
+  Fixpoint map_IndexedQS_idx_boundi'
+        {indices}
+  : forall
+      n
+      (Index : ilist
+                 (fun ns : NamedSchema =>
+                    SearchUpdateTerms (schemaHeading (relSchema ns)))
+                 indices)
+      idx, 
+      nth_error (map relName indices) n = Some idx
+      -> nth_error
+        (map ADTSigname (Build_IndexedQueryStructure_Impl_Sigs Index))
+        n = Some idx.
+  Proof.
+    refine (match indices with
+              | nil => _
+              | ns :: indices' =>
+                fun n => 
+                  match n return
+                        forall
+                          (Index : ilist
+                                     (fun ns : NamedSchema =>
+                                        SearchUpdateTerms (schemaHeading (relSchema ns)))
+                                     (ns :: indices'))
+                          idx,
+                          nth_error (map relName (ns :: indices')) n = Some idx
+                          -> nth_error (map ADTSigname (Build_IndexedQueryStructure_Impl_Sigs Index)) n = Some idx
+                  with
+                    | 0 => fun Index idx nth_n => nth_n
+                    | S n' => fun Index => (map_IndexedQS_idx_boundi' indices' n' (ilist_tl Index))
+                  end
+            end);
+    simpl; intros; try discriminate; eauto.
+  Defined.
+  
+  Definition map_IndexedQS_idx'
+             indices
+             (Index : ilist (fun ns : NamedSchema => SearchUpdateTerms (schemaHeading (relSchema ns))) indices )
+             (idx : BoundedIndex (map relName indices))
+  : BoundedIndex
+                      (map ADTSigname
+                           (Build_IndexedQueryStructure_Impl_Sigs Index)) := 
+    {| bindex := bindex idx;
+       indexb := {| ibound := ibound (indexb idx);
+                    boundi := map_IndexedQS_idx_boundi' _ Index (boundi (indexb idx))|} |}.
+
+  Lemma ith_Build_IndexedQueryStructure_Impl_Sigs_eq
+        {indices}
+  : forall
+      (Index : ilist (fun ns : NamedSchema => SearchUpdateTerms (schemaHeading (relSchema ns))) indices )
+      (idx : BoundedIndex
+               (map ADTSigname
+                    (Build_IndexedQueryStructure_Impl_Sigs Index))),
+      (BagSig (@Tuple (schemaHeading (relSchema ((nth_Bounded relName indices (map_IndexedQS_idx Index idx))))))
+              (BagSearchTermType
+                 (ith_Bounded relName Index (map_IndexedQS_idx Index idx)))
+              (BagUpdateTermType
+                 (ith_Bounded relName Index (map_IndexedQS_idx Index idx))))
+      = namedADTSig
+          (nth_Bounded ADTSigname (Build_IndexedQueryStructure_Impl_Sigs Index) idx).
+  Proof.
+    destruct idx as [idx [n nth_n]].
+    revert Index idx n nth_n.
+    induction indices; destruct n; simpl; intros; try discriminate; eauto.
+    eapply (IHindices (ilist_tl Index) idx n nth_n).
+  Defined.
+
+  Lemma ith_Build_IndexedQueryStructure_Impl_Specs_eq
+        {indices}
+  : forall
+      (Index : ilist (fun ns : NamedSchema => SearchUpdateTerms (schemaHeading (relSchema ns))) indices )
+      (idx : BoundedIndex
+               (map ADTSigname
+                    (Build_IndexedQueryStructure_Impl_Sigs Index))),
+      ith_Bounded ADTSigname (Build_IndexedQueryStructure_Impl_Specs Index) idx = 
+  eq_rect _ ADT
+          (@BagSpec (@Tuple (schemaHeading (relSchema (@nth_Bounded NamedSchema string relName
+                                                                    indices (map_IndexedQS_idx Index idx)))))
+                    (BagSearchTermType (ith_Bounded _ Index (map_IndexedQS_idx Index idx)))
+                    (BagUpdateTermType (ith_Bounded _ Index (map_IndexedQS_idx Index idx)))
+                    (BagMatchSearchTerm (ith_Bounded _ Index (map_IndexedQS_idx Index idx)))
+                    (BagApplyUpdateTerm (ith_Bounded _ Index (map_IndexedQS_idx Index idx))))
+                    _ (ith_Build_IndexedQueryStructure_Impl_Sigs_eq Index idx).
+  Proof.
+    destruct idx as [idx [n nth_n]].
+    revert Index idx n nth_n.
+    induction indices; destruct n; simpl; intros; try discriminate; eauto.
+    eapply (IHindices (ilist_tl Index) idx n nth_n).
+  Defined.
+        
+  Definition map_IndexedQS_Rep 
+             {indices}
+             (Index : ilist (fun ns : NamedSchema => SearchUpdateTerms (schemaHeading (relSchema ns))) indices )
+             idx
+             (rep : @IndexedEnsemble
+                      (@Tuple
+                         (schemaHeading
+                            (relSchema
+                               (@nth_Bounded NamedSchema string relName
+                                             indices (map_IndexedQS_idx Index idx) )))))
+  : Rep
+      (ith_Bounded ADTSigname
+                   (Build_IndexedQueryStructure_Impl_Specs Index) idx).
+  Proof.
+    destruct idx as [idx [n nth_n]].
+    revert Index idx n nth_n rep.
+    induction indices; destruct n; simpl; intros; try discriminate; eauto.
+    eapply IHindices; eauto.
+  Defined.
+
+  Definition map_IndexedQS_Rep'
+             {indices}
+             (Index : ilist (fun ns : NamedSchema => SearchUpdateTerms (schemaHeading (relSchema ns))) indices )
+             idx
+             (rep : Rep
+                      (ith_Bounded ADTSigname
+                                   (Build_IndexedQueryStructure_Impl_Specs Index)
+                                   (map_IndexedQS_idx' Index idx)))
+  : @IndexedEnsemble
+      (@Tuple
+         (schemaHeading
+            (relSchema
+               (@nth_Bounded NamedSchema string relName
+                             indices idx )))).
+  Proof.
+    destruct idx as [idx [n nth_n]].
+    revert Index idx n nth_n rep.
+    induction indices; destruct n; simpl; intros; try discriminate; eauto.
+    eapply (IHindices (ilist_tl Index)); eauto.
+  Defined.
+    
+  Definition Build_IndexedQueryStructure_Impl_AbsR
+             {qs_schema : QueryStructureSchema}
+             (Index : ilist (fun ns : NamedSchema => SearchUpdateTerms (schemaHeading (relSchema ns))) (qschemaSchemas qs_schema) )
+             (DelegateImpls : ilist (fun ns => cADT (namedADTSig ns))
+                                     (Build_IndexedQueryStructure_Impl_Sigs Index))
+             (ValidImpl :
+                forall idx,
+                  refineADT (ith_Bounded ADTSigname
+                                         (Build_IndexedQueryStructure_Impl_Specs Index) idx)
+                            (LiftcADT (ith_Bounded ADTSigname DelegateImpls idx)))
+             (r_o : IndexedQueryStructure qs_schema Index)
+             (r_n : Build_IndexedQueryStructure_Impl_cRep Index DelegateImpls)
+  : Prop := 
+    forall idx,
+      AbsR (ValidImpl idx)
+           (map_IndexedQS_Rep Index idx (GetIndexedRelation r_o (map_IndexedQS_idx Index idx)))
+           (i2th_Bounded ADTSigname r_n idx).
+
+  Definition map_IndexedQS_Rep''
+             {indices}
+             (Index : ilist (fun ns : NamedSchema => SearchUpdateTerms (schemaHeading (relSchema ns))) indices )
+             idx
+             (rep : @IndexedEnsemble
+                      (@Tuple
+                         (schemaHeading
+                            (relSchema
+                               (@nth_Bounded NamedSchema string relName
+                                             indices idx)))))
+  : Rep
+      (ith_Bounded ADTSigname
+                   (Build_IndexedQueryStructure_Impl_Specs Index) (map_IndexedQS_idx' Index idx)).
+  Proof.
+    destruct idx as [idx [n nth_n]].
+    revert Index idx n nth_n rep.
+    induction indices; destruct n; simpl; intros; try discriminate; eauto.
+    eapply IHindices; eauto.
+  Defined.
+
+  Definition Build_IndexedQueryStructure_Impl_AbsR''
+             {qs_schema : QueryStructureSchema}
+             (Index : ilist (fun ns : NamedSchema => SearchUpdateTerms (schemaHeading (relSchema ns))) (qschemaSchemas qs_schema) )
+             (DelegateImpls : ilist (fun ns => cADT (namedADTSig ns))
+                                     (Build_IndexedQueryStructure_Impl_Sigs Index))
+             (ValidImpl :
+                forall idx : BoundedIndex (map relName (qschemaSchemas qs_schema)),
+                  refineADT (ith_Bounded ADTSigname
+                                         (Build_IndexedQueryStructure_Impl_Specs Index) (map_IndexedQS_idx' Index idx))
+                            (LiftcADT (ith_Bounded ADTSigname DelegateImpls (map_IndexedQS_idx' Index idx))))
+             (r_o : IndexedQueryStructure qs_schema Index)
+             (r_n : Build_IndexedQueryStructure_Impl_cRep Index DelegateImpls)
+  : Prop := 
+    forall idx,
+      AbsR (ValidImpl idx)
+           (map_IndexedQS_Rep'' Index idx (GetIndexedRelation r_o idx))
+           (i2th_Bounded ADTSigname r_n (map_IndexedQS_idx' Index idx)).
+
+  Definition CallBagImplMethod
+             {qs_schema : QueryStructureSchema}
+             (Index : ilist (fun ns : NamedSchema => SearchUpdateTerms (schemaHeading (relSchema ns))) (qschemaSchemas qs_schema) )
+             (DelegateImpls : ilist (fun ns => cADT (namedADTSig ns))
+                                    (Build_IndexedQueryStructure_Impl_Sigs Index))
+             idx midx
+             (r_n : Build_IndexedQueryStructure_Impl_cRep Index DelegateImpls) :=
+    cMethods (ith_Bounded ADTSigname DelegateImpls idx) midx (i2th_Bounded _ r_n idx).
+
+  Definition CallBagImplConstructor
+             {qs_schema : QueryStructureSchema}
+             (Index : ilist (fun ns : NamedSchema => SearchUpdateTerms (schemaHeading (relSchema ns))) (qschemaSchemas qs_schema) )
+             (DelegateImpls : ilist (fun ns => cADT (namedADTSig ns))
+                                    (Build_IndexedQueryStructure_Impl_Sigs Index))
+             idx midx :=
+    cConstructors (ith_Bounded ADTSigname DelegateImpls idx) midx .
+
+  Fixpoint Build_IndexedQueryStructure_Impl_midx
+           {indices}
+           (P : ADTSig -> Type)
+  : forall (Index : ilist (fun ns : NamedSchema => SearchUpdateTerms (schemaHeading (relSchema ns))) indices)
+             ridx
+             (midx : P
+                       (BagSig (@Tuple (schemaHeading
+                            (relSchema
+                               (@nth_Bounded NamedSchema string relName
+                                             indices (map_IndexedQS_idx Index ridx ) ))))
+                               (BagSearchTermType
+                                  (ith_Bounded relName Index (map_IndexedQS_idx Index ridx)))
+                               (BagUpdateTermType
+                                  (ith_Bounded relName Index (map_IndexedQS_idx Index ridx))))),
+      P
+        (namedADTSig
+           (nth_Bounded ADTSigname (Build_IndexedQueryStructure_Impl_Sigs Index)
+                        ridx)) := 
+    match indices return
+          forall (Index : ilist
+                            (fun ns : NamedSchema =>
+                               SearchUpdateTerms (schemaHeading (relSchema ns)))
+                            indices)
+                 (ridx : BoundedIndex
+                           (map ADTSigname (Build_IndexedQueryStructure_Impl_Sigs Index)))
+                 (midx : P
+                       (BagSig (@Tuple (schemaHeading
+                            (relSchema
+                               (@nth_Bounded NamedSchema string relName
+                                             indices (map_IndexedQS_idx Index ridx ) ))))
+                               (BagSearchTermType
+                                  (ith_Bounded relName Index (map_IndexedQS_idx Index ridx)))
+                               (BagUpdateTermType
+                                  (ith_Bounded relName Index (map_IndexedQS_idx Index ridx))))),
+      P
+        (namedADTSig
+           (nth_Bounded ADTSigname (Build_IndexedQueryStructure_Impl_Sigs Index)
+                        ridx))
+    with
+      | nil => fun _ ridx => BoundedIndex_nil _ ridx
+      | ns :: indices' =>
+        fun Index ridx =>  
+          match ridx with
+            | {| bindex := ridx;
+                 indexb := {|ibound := n;
+                             boundi := nth_n |}|} => 
+              match n return
+                    forall
+                      (Index' : ilist
+                                  (fun ns : NamedSchema =>
+                                     SearchUpdateTerms (schemaHeading (relSchema ns))) (ns :: indices'))
+                      ridx nth_n,
+                      let idx := {| bindex := ridx;
+                                    indexb := {|ibound := n;
+                                                boundi := nth_n |}|} in 
+                      P
+                                (BagSig (@Tuple (schemaHeading
+                                                   (relSchema
+                                                      (@nth_Bounded NamedSchema string relName
+                                                                    (ns :: indices') (map_IndexedQS_idx Index' idx ) ))))
+                                        (BagSearchTermType
+                                           (ith_Bounded relName Index' (map_IndexedQS_idx Index' idx)))
+                                        (BagUpdateTermType
+                                           (ith_Bounded relName Index' (map_IndexedQS_idx Index' idx)))) -> 
+                      P
+                        (namedADTSig
+                           (nth_Bounded ADTSigname (Build_IndexedQueryStructure_Impl_Sigs Index')
+                                        {| bindex := ridx;
+                                           indexb := {|ibound := n;
+                                                       boundi := nth_n |}|}))
+              with
+                | 0 => fun Index idx nth_n midx => midx
+                | S n' => fun Index idx nth_n midx =>
+                            (@Build_IndexedQueryStructure_Impl_midx
+                               indices' P (ilist_tl Index)
+                               {| bindex := idx;
+                                  indexb := {|ibound := n';
+                                              boundi := nth_n |}|}
+                               midx)
+              end Index ridx nth_n 
+                            end
+         end.  
+
+
+(*fst
+    (MethodDomCod
+       (BagSig Tuple (BagSearchTermType (ith_Bounded relName Index ridx))
+          (BagUpdateTermType (ith_Bounded relName Index ridx))) midx)"
+ while it is expected to have type
+ "fst
+    (MethodDomCod
+       (namedADTSig
+          (nth_Bounded ADTSigname
+             (Build_IndexedQueryStructure_Impl_Sigs Index) ridx')) midx')" *)
+  
+  Definition Build_IndexedQueryStructure_Impl_MethodDom
+           {indices}
+  : forall (Index : ilist (fun ns : NamedSchema => SearchUpdateTerms (schemaHeading (relSchema ns))) indices)
+           ridx
+           midx,
+      fst (MethodDomCod
+             (BagSig (@Tuple (schemaHeading (relSchema (nth_Bounded relName indices  ridx))))
+                     (BagSearchTermType
+                        (ith_Bounded relName Index ridx))
+                     (BagUpdateTermType
+                        (ith_Bounded relName Index ridx)))
+             midx)
+    -> fst
+        (MethodDomCod
+           (namedADTSig
+              (nth_Bounded ADTSigname
+                           (Build_IndexedQueryStructure_Impl_Sigs Index) (map_IndexedQS_idx' Index ridx)))
+           (Build_IndexedQueryStructure_Impl_midx MethodIndex Index (map_IndexedQS_idx' Index ridx) midx)).
+  Proof.
+    destruct ridx as [idx [n nth_n]]; revert Index idx n nth_n.
+    induction indices.
+  - destruct n; simpl; discriminate.
+  - destruct n; simpl; eauto.
+    intros; eapply (IHindices (ilist_tl Index) idx n nth_n); eauto.
+  Defined.
+
+  Definition Build_IndexedQueryStructure_Impl_MethodCod
+           {indices}
+  : forall (Index : ilist (fun ns : NamedSchema => SearchUpdateTerms (schemaHeading (relSchema ns))) indices)
+           ridx
+           midx,
+      snd
+        (MethodDomCod
+           (namedADTSig
+              (nth_Bounded ADTSigname
+                           (Build_IndexedQueryStructure_Impl_Sigs Index) (map_IndexedQS_idx' Index ridx)))
+           (Build_IndexedQueryStructure_Impl_midx MethodIndex Index (map_IndexedQS_idx' Index ridx) midx))
+  ->       snd (MethodDomCod
+             (BagSig (@Tuple (schemaHeading (relSchema (nth_Bounded relName indices  ridx))))
+                     (BagSearchTermType
+                        (ith_Bounded relName Index ridx))
+                     (BagUpdateTermType
+                        (ith_Bounded relName Index ridx)))
+             midx)
+.
+  Proof.
+    destruct ridx as [idx [n nth_n]]; revert Index idx n nth_n.
+    induction indices.
+  - destruct n; simpl; discriminate.
+  - destruct n; simpl; eauto.
+    intros; eapply (IHindices (ilist_tl Index) idx n nth_n); eauto.
+  Defined.
+
+Lemma ith_Build_IndexedQueryStructure_Impl_Methods
+        {indices}
+  : forall
+      (Index : ilist (fun ns : NamedSchema => SearchUpdateTerms (schemaHeading (relSchema ns))) indices )
+      (idx : BoundedIndex
+               (map ADTSigname
+                    (Build_IndexedQueryStructure_Impl_Sigs Index))),
+      Methods (ith_Bounded ADTSigname (Build_IndexedQueryStructure_Impl_Specs Index) idx) = 
+      eq_rect _ (fun r => forall idx, methodType (Rep r) _ _ )
+              (Methods (eq_rect _ ADT
+                                (@BagSpec (@Tuple (schemaHeading (relSchema (@nth_Bounded NamedSchema string relName
+                                                                                          indices (map_IndexedQS_idx Index idx)))))
+                                          (BagSearchTermType (ith_Bounded _ Index (map_IndexedQS_idx Index idx)))
+                                          (BagUpdateTermType (ith_Bounded _ Index (map_IndexedQS_idx Index idx)))
+                                          (BagMatchSearchTerm (ith_Bounded _ Index (map_IndexedQS_idx Index idx)))
+                                          (BagApplyUpdateTerm (ith_Bounded _ Index (map_IndexedQS_idx Index idx))))
+                                _ (ith_Build_IndexedQueryStructure_Impl_Sigs_eq Index idx)))
+              _ (eq_sym (ith_Build_IndexedQueryStructure_Impl_Specs_eq Index idx)).
+  Proof.
+    destruct idx as [idx [n nth_n]].
+    revert Index idx n nth_n.
+    induction indices; destruct n; simpl; intros; try discriminate; eauto.
+    eapply (IHindices (ilist_tl Index) idx n nth_n).
+  Defined.
+  
+  Lemma refine_Mapped_Methods
+        {indices}
+        (Index : ilist (fun ns : NamedSchema => SearchUpdateTerms (schemaHeading (relSchema ns))) (indices) )
+  :  forall
+      ridx,
+      forall
+        (r_o : @IndexedEnsemble (@Tuple (schemaHeading (relSchema (nth_Bounded relName indices ridx)))))
+      midx 
+      d r s,
+        let ridx' := map_IndexedQS_idx' Index ridx in 
+        let midx' := Build_IndexedQueryStructure_Impl_midx MethodIndex Index ridx' midx in
+        let d' := Build_IndexedQueryStructure_Impl_MethodDom Index ridx _ d in
+Methods
+     (ith_Bounded ADTSigname (Build_IndexedQueryStructure_Impl_Specs Index) ridx') midx'
+     (map_IndexedQS_Rep'' Index ridx r_o) d'
+     ↝ (r, s) ->
+Methods
+  (BagSpec (BagMatchSearchTerm (ith_Bounded relName Index ridx))
+           (BagApplyUpdateTerm (ith_Bounded relName Index ridx))) midx r_o d
+   ↝ (map_IndexedQS_Rep' Index ridx r,
+     Build_IndexedQueryStructure_Impl_MethodCod Index ridx midx s).
+  Proof.
+    intros; pose proof (ith_Build_IndexedQueryStructure_Impl_Methods Index ridx') as H';
+    rewrite H' in H; revert H; clear H'.
+    unfold d', midx', ridx' in *; clear ridx' midx' d'.
+    revert r_o d r s.
+    intro; eapply (Iterate_Dep_Type_BoundedIndex_equiv_1) with (idx := midx);
+    simpl.
+    intuition;
+      simpl in *;
+      first [revert midx r_o d r s H
+            | revert midx r_o b a r s H ];
+    try (destruct ridx as [idx [n nth_n]];
+      revert idx n nth_n;
+      unfold IndexedQueryStructure, GetIndexedRelation in *;
+      unfold list_ind, list_rect in *;
+      induction indices; destruct n; simpl; try (intros; discriminate); eauto;
+      eapply IHindices).
+  Qed.
+  
+  Lemma refine_BagImplMethods
+        {qs_schema : QueryStructureSchema}
+        (Index : ilist (fun ns : NamedSchema => SearchUpdateTerms (schemaHeading (relSchema ns))) (qschemaSchemas qs_schema) )
+        (DelegateImpls : ilist (fun ns => cADT (namedADTSig ns))
+                               (Build_IndexedQueryStructure_Impl_Sigs Index))
+        ValidImpl
+  :  forall (r_o : IndexedQueryStructure qs_schema Index)
+            (r_n : Build_IndexedQueryStructure_Impl_cRep Index DelegateImpls)
+            ridx,
+            let ridx' := map_IndexedQS_idx' Index ridx in 
+            forall (midx : MethodIndex
+                     (BagSig Tuple
+                             (BagSearchTermType
+                                (ith_Bounded relName Index (map_IndexedQS_idx Index ridx')))
+                             (BagUpdateTermType
+                                (ith_Bounded relName Index (map_IndexedQS_idx Index ridx')))))
+                   (d : fst
+                          (MethodDomCod
+                             (BagSig (@Tuple (schemaHeading (relSchema (nth_Bounded relName (qschemaSchemas qs_schema) ridx))))
+                                     (BagSearchTermType (ith_Bounded relName Index ridx))
+                                     (BagUpdateTermType (ith_Bounded relName Index ridx))) midx)),
+       let midx' := Build_IndexedQueryStructure_Impl_midx MethodIndex Index ridx' midx in
+       let d' := Build_IndexedQueryStructure_Impl_MethodDom Index ridx _ d in
+       Build_IndexedQueryStructure_Impl_AbsR'' ValidImpl r_o r_n ->
+       exists r_o',
+         AbsR (ValidImpl ridx) r_o' (fst (CallBagImplMethod ridx' midx' r_n d'))
+         /\ refine (CallBagMethod ridx midx r_o d)
+                   (ret (map_IndexedQS_Rep' _ _ r_o',
+                         Build_IndexedQueryStructure_Impl_MethodCod Index ridx _
+                                                                    (snd (CallBagImplMethod (map_IndexedQS_idx' Index ridx) midx' r_n d')))).
+    intros.
+    pose proof (ADTRefinementPreservesMethods (ValidImpl ridx) midx'
+                                              (map_IndexedQS_Rep'' Index ridx
+                                                                 (GetIndexedRelation r_o ridx))
+                                              (i2th_Bounded _ r_n ridx') d' (H ridx) (ReturnComputes _)).
+    Local Arguments map_IndexedQS_Rep : simpl never.
+    inversion_by computes_to_inv; subst.
+    exists (fst x);
+      unfold CallBagImplMethod; simpl in *. 
+      split; simpl.
+      - pose proof (f_equal fst H3) as eq_x0; simpl in eq_x0.
+        rewrite eq_x0 in H2; simpl in H2; apply H2.
+    - pose proof (f_equal snd H3) as eq_x; simpl in eq_x.
+      assert (refine (CallBagMethod ridx midx r_o d)
+                     (ret
+                        (map_IndexedQS_Rep' Index ridx (fst x),
+                         Build_IndexedQueryStructure_Impl_MethodCod Index ridx midx (snd x))));
+        [ | rewrite eq_x in H0;  eapply H0 ].
+      intros v Comp_v; simpl in *; inversion_by computes_to_inv; subst.
+      destruct x; simpl @fst in *; simpl @snd in *.
+      unfold ridx' in *.
+      revert H1.
+      Local Transparent CallBagMethod.
+      eapply refine_Mapped_Methods.
+  Qed.
+
+  (*Fixpoint Build_IndexedQueryStructure_Impl_ConstructorDom
+           {indices}
+           {struct indices}
+  : forall (Index : ilist (fun ns : NamedSchema => SearchUpdateTerms (schemaHeading (relSchema ns))) indices)
+             ridx
+             (midx : ConstructorIndex
+                       (BagSig (@Tuple (schemaHeading
+                            (relSchema
+                               (@nth_Bounded NamedSchema string relName
+                                             indices (map_IndexedQS_idx Index ridx ) ))))
+                               (BagSearchTermType
+                                  (ith_Bounded relName Index (map_IndexedQS_idx Index ridx)))
+                               (BagUpdateTermType
+                                  (ith_Bounded relName Index (map_IndexedQS_idx Index ridx))))),
+      (ConstructorDom
+             (BagSig Tuple
+                     (BagSearchTermType
+                        (ith_Bounded relName Index (map_IndexedQS_idx Index ridx)))
+                     (BagUpdateTermType
+                        (ith_Bounded relName Index (map_IndexedQS_idx Index ridx))))
+             midx) -> 
+      (ConstructorDom
+             (namedADTSig
+                (nth_Bounded ADTSigname (Build_IndexedQueryStructure_Impl_Sigs Index)
+                             ridx))
+             (Build_IndexedQueryStructure_Impl_midx ConstructorIndex Index ridx midx)) := 
+    match indices return
+          forall (Index : ilist
+                            (fun ns : NamedSchema =>
+                               SearchUpdateTerms (schemaHeading (relSchema ns)))
+                            indices)
+                 (ridx : BoundedIndex
+                           (map ADTSigname (Build_IndexedQueryStructure_Impl_Sigs Index)))
+                 (midx : ConstructorIndex
+                       (BagSig (@Tuple (schemaHeading
+                            (relSchema
+                               (@nth_Bounded NamedSchema string relName
+                                             indices (map_IndexedQS_idx Index ridx ) ))))
+                               (BagSearchTermType
+                                  (ith_Bounded relName Index (map_IndexedQS_idx Index ridx)))
+                               (BagUpdateTermType
+                                  (ith_Bounded relName Index (map_IndexedQS_idx Index ridx))))),
+            (ConstructorDom
+                   (BagSig Tuple
+                           (BagSearchTermType
+                              (ith_Bounded relName Index (map_IndexedQS_idx Index ridx)))
+                     (BagUpdateTermType
+                        (ith_Bounded relName Index (map_IndexedQS_idx Index ridx))))
+                   midx) -> 
+            (ConstructorDom
+                   (namedADTSig
+                      (nth_Bounded ADTSigname (Build_IndexedQueryStructure_Impl_Sigs Index)
+                                   ridx))
+                   (Build_IndexedQueryStructure_Impl_midx ConstructorIndex Index ridx midx))
+    with
+      | nil => fun _ ridx => BoundedIndex_nil _ ridx
+      | ns :: indices' =>
+        fun Index ridx =>  
+          match ridx with
+            | {| bindex := ridx;
+                 indexb := {|ibound := n;
+                             boundi := nth_n |}|} => 
+              match n return
+                    forall
+                      (Index' : ilist
+                                  (fun ns : NamedSchema =>
+                                     SearchUpdateTerms (schemaHeading (relSchema ns))) (ns :: indices'))
+                      ridx nth_n,
+                      let idx := {| bindex := ridx;
+                                    indexb := {|ibound := n;
+                                                boundi := nth_n |}|} in 
+                      forall (midx : ConstructorIndex (BagSig (@Tuple (schemaHeading
+                                                     (relSchema
+                                                        (@nth_Bounded NamedSchema string relName
+                                                                      (ns :: indices') (map_IndexedQS_idx Index' idx ) ))))
+                                          (BagSearchTermType
+                                             (ith_Bounded relName Index' (map_IndexedQS_idx Index' idx)))
+                                          (BagUpdateTermType
+                                             (ith_Bounded relName Index' (map_IndexedQS_idx Index' idx))))),
+                      (ConstructorDom
+                             (BagSig Tuple
+                                     (BagSearchTermType
+                                        (ith_Bounded relName Index' (map_IndexedQS_idx Index' idx)))
+                                     (BagUpdateTermType
+                                        (ith_Bounded relName Index' (map_IndexedQS_idx Index' idx))))
+                             midx) -> 
+                      (ConstructorDom
+                             (namedADTSig
+                                (nth_Bounded ADTSigname (Build_IndexedQueryStructure_Impl_Sigs Index')
+                                             idx))
+                             (Build_IndexedQueryStructure_Impl_midx ConstructorIndex Index' idx midx))
+              with
+                | 0 => fun Index idx nth_n midx d => d
+                | S n' => fun Index idx nth_n midx d =>
+                            (@Build_IndexedQueryStructure_Impl_ConstructorDom
+                               indices' (ilist_tl Index)
+                               {| bindex := idx;
+                                  indexb := {|ibound := n';
+                                              boundi := nth_n |}|}
+                               midx d)
+              end Index ridx nth_n 
+                            end
+         end.
+
+  Lemma ith_Build_IndexedQueryStructure_Impl_Constructors
+        {indices}
+  : forall
+      (Index : ilist (fun ns : NamedSchema => SearchUpdateTerms (schemaHeading (relSchema ns))) indices )
+      (idx : BoundedIndex
+               (map ADTSigname
+                    (Build_IndexedQueryStructure_Impl_Sigs Index))),
+      Constructors (ith_Bounded ADTSigname (Build_IndexedQueryStructure_Impl_Specs Index) idx) = 
+      eq_rect _ (fun r => forall idx, constructorType (Rep r) _ )
+              (Constructors (eq_rect _ ADT
+                                (@BagSpec (@Tuple (schemaHeading (relSchema (@nth_Bounded NamedSchema string relName
+                                                                                          indices (map_IndexedQS_idx Index idx)))))
+                                          (BagSearchTermType (ith_Bounded _ Index (map_IndexedQS_idx Index idx)))
+                                          (BagUpdateTermType (ith_Bounded _ Index (map_IndexedQS_idx Index idx)))
+                                          (BagMatchSearchTerm (ith_Bounded _ Index (map_IndexedQS_idx Index idx)))
+                                          (BagApplyUpdateTerm (ith_Bounded _ Index (map_IndexedQS_idx Index idx))))
+                                _ (ith_Build_IndexedQueryStructure_Impl_Sigs_eq Index idx)))
+              _ (eq_sym (ith_Build_IndexedQueryStructure_Impl_Specs_eq Index idx)).
+  Proof.
+    destruct idx as [idx [n nth_n]].
+    revert Index idx n nth_n.
+    induction indices; destruct n; simpl; intros; try discriminate; eauto.
+    eapply (IHindices (ilist_tl Index) idx n nth_n).
+  Defined.
+
+  Lemma refine_Mapped_Constructors
+        {indices}
+        (Index : ilist (fun ns : NamedSchema => SearchUpdateTerms (schemaHeading (relSchema ns))) (indices) )
+  :  forall
+      ridx
+      (midx : ConstructorIndex
+                (BagSig Tuple
+                        (BagSearchTermType
+                           (ith_Bounded relName Index (map_IndexedQS_idx Index ridx)))
+                        (BagUpdateTermType
+                           (ith_Bounded relName Index (map_IndexedQS_idx Index ridx)))))
+      d r,
+      Constructors (ith_Bounded ADTSigname (Build_IndexedQueryStructure_Impl_Specs Index) ridx) (Build_IndexedQueryStructure_Impl_midx ConstructorIndex Index ridx midx)
+                   (Build_IndexedQueryStructure_Impl_ConstructorDom Index ridx midx d)
+                   ↝ r ->
+      Constructors
+        (BagSpec (BagMatchSearchTerm (ith_Bounded relName Index (map_IndexedQS_idx Index ridx)))
+                 (BagApplyUpdateTerm (ith_Bounded relName Index (map_IndexedQS_idx Index ridx)))) midx d
+   ↝ map_IndexedQS_Rep' Index ridx r.
+  Proof.
+    intros; pose proof (ith_Build_IndexedQueryStructure_Impl_Constructors Index ridx) as H';
+      simpl ith_Bounded in *; rewrite H' in H; revert H.
+    clear H'.
+    revert d r.
+    eapply Iterate_Dep_Type_BoundedIndex_equiv_1 with (idx := midx).
+    simpl; intuition.
+    simpl in *.
+    revert midx d r H.
+    destruct ridx as [idx [n nth_n]];
+      revert idx n nth_n;
+      unfold IndexedQueryStructure, GetIndexedRelation in *;
+      unfold list_ind, list_rect in *;
+      induction indices; destruct n; simpl; try (intros; discriminate); eauto;
+      eapply IHindices.
+  Qed.
+
+  Check refine_BagImplMethods.
+  Check CallBagImplConstructor.
+    
+  Lemma refine_BagImplConstructors
+        {qs_schema : QueryStructureSchema}
+        (Index : ilist (fun ns : NamedSchema => SearchUpdateTerms (schemaHeading (relSchema ns))) (qschemaSchemas qs_schema) )
+        (DelegateImpls : ilist (fun ns => cADT (namedADTSig ns))
+                               (Build_IndexedQueryStructure_Impl_Sigs Index))
+        (ValidImpl : forall
+                        idx : BoundedIndex
+                                (map ADTSigname
+                                   (Build_IndexedQueryStructure_Impl_Sigs
+                                      Index)),
+                      refineADT
+                        (ith_Bounded ADTSigname
+                           (Build_IndexedQueryStructure_Impl_Specs Index)
+                           idx)
+                        (LiftcADT (ith_Bounded ADTSigname DelegateImpls idx)))
+  :  forall (ridx : BoundedIndex
+                   (map ADTSigname
+                      (Build_IndexedQueryStructure_Impl_Sigs Index)))
+            (midx : ConstructorIndex
+                     (BagSig Tuple
+                             (BagSearchTermType
+                                (ith_Bounded relName Index (map_IndexedQS_idx Index ridx)))
+                             (BagUpdateTermType
+                                (ith_Bounded relName Index (map_IndexedQS_idx Index ridx)))))
+            d,
+       let midx' := Build_IndexedQueryStructure_Impl_midx ConstructorIndex Index ridx midx in
+       let d' := Build_IndexedQueryStructure_Impl_ConstructorDom Index ridx midx d in
+       exists r_o',
+         AbsR (ValidImpl ridx) r_o' (CallBagImplConstructor _ DelegateImpls ridx midx' d')
+         /\ refine (CallBagConstructor _ _ (map_IndexedQS_idx Index ridx) midx d)
+                   (ret (map_IndexedQS_Rep' _ _ r_o')) .
+  Proof.
+    intros.
+    pose proof (ADTRefinementPreservesConstructors (ValidImpl ridx) midx'
+                                                   d' (ReturnComputes _)).
+    inversion_by computes_to_inv; subst.
+    exists x;
+      unfold CallBagImplConstructor; simpl in *; split; simpl.
+    - eassumption.
+    - intros v Comp_v; simpl in *; inversion_by computes_to_inv; subst.
+      Local Transparent CallBagConstructor.
+      eapply refine_Mapped_Constructors; eauto.
+  Qed.
+ *)
+
+  Definition Build_IndexedQueryStructure_Impl_AbsR'
+             {qs_schema : QueryStructureSchema}
+             (Index : ilist (fun ns : NamedSchema => SearchUpdateTerms (schemaHeading (relSchema ns))) (qschemaSchemas qs_schema) )
+             (DelegateImpls : ilist (fun ns => cADT (namedADTSig ns))
+                                     (Build_IndexedQueryStructure_Impl_Sigs Index))
+             (ValidImpl :
+                forall idx,
+                  refineADT (ith_Bounded ADTSigname
+                                         (Build_IndexedQueryStructure_Impl_Specs Index) idx)
+                            (LiftcADT (ith_Bounded ADTSigname DelegateImpls idx)))
+             (r_o : IndexedQueryStructure qs_schema Index)
+             (r_n : Build_IndexedQueryStructure_Impl_cRep Index DelegateImpls)
+  : Prop := 
+      @Build_IndexedQueryStructure_Impl_AbsR''
+        qs_schema Index DelegateImpls
+        (fun idx => ValidImpl (map_IndexedQS_idx' Index idx))
+        r_o
+        r_n.
+  
+  FullySharpenEachMethod
+    (Build_IndexedQueryStructure_Impl_Sigs Index)
+    (Build_IndexedQueryStructure_Impl_Specs Index)
+    (Build_IndexedQueryStructure_Impl_cRep Index)
+    (@Build_IndexedQueryStructure_Impl_AbsR' BookStoreSchema Index).
+
+  Focus 3.
+
+  intros.
+  Opaque CallBagMethod.
+  simplify with monad laws.
+  simpl in *. unfold Build_IndexedQueryStructure_Impl_AbsR' in *.
+  match goal with
+      H : Build_IndexedQueryStructure_Impl_AbsR'' (qs_schema := ?qs_schema) ?ValidImpl ?r_o ?r_n
+      |- context[CallBagMethod (BagIndexKeys := ?Index') ?ridx ?midx ?r_o ?d] =>
+      let r_o' := fresh "r_o'" in
+      let AbsR_r_o' := fresh "AbsR_r_o'" in 
+      let refines_r_o := fresh "refines_r_o'" in 
+      destruct (@refine_BagImplMethods qs_schema Index' _ ValidImpl r_o r_n ridx midx d H) as [r_o' [AbsR_r_o' refines_r_o']]; 
+      unfold map_IndexedQS_idx' in refines_r_o', AbsR_r_o'; simpl in refines_r_o', AbsR_r_o';
+      setoid_rewrite refines_r_o'; simpl in *; simplify with monad laws; simpl
+  end.
+
+  refine pick val _.
+
+  Focus 2.
+  unfold Build_IndexedQueryStructure_Impl_AbsR''.
+  
+  
+  
+  simpl.
+  Set Printing Implicit.
+  idtac.
+  rewrite H2.
+  
+  pose (e q i _ r i0 b b0 b1 p).
+
+
+  
+  Focus 3.
+  
+    [BagSig Book (BuildSearchTermFromAttributes BookSearchTerm);
                            BagSig Order (BuildSearchTermFromAttributes OrderSearchTerm)]
                          (icons _ (BagSpec (SearchTermFromAttributesMatcher BookSearchTerm))
                          (icons _ (BagSpec (SearchTermFromAttributesMatcher OrderSearchTerm))
