src/QueryStructure/Implementation/Operations/BagADT/Refinements.v
@@ -49,9 +49,11 @@ Section BagsQueryStructureRefinements.
     econstructor.
     unfold IndexedQueryStructure, DelegateToBag_AbsR, GetIndexedRelation.
     unfold GetUnConstrRelation.
-    unfold DropQSConstraints, QSEmptySpec.
+    unfold DropQSConstraints, QSEmptySpec; split.
     intros; rewrite <- ith_Bounded_imap, ith_Bounded_BuildEmptyRelations,
     i2th_Bounded_Initialize_IndexedQueryStructure; eauto.
+    intros; eexists [];
+    apply EnsembleIndexedListEquivalence_Empty.
   Qed.
 
   Definition UpdateIndexedRelation
@@ -78,21 +80,85 @@ Section BagsQueryStructureRefinements.
   Qed.
 
   (* Cross product of lists using heterogenous lists. *)
-    Definition Join_Lists
+  Definition Join_Lists
              {A : Type}
              {f : A -> Type}
              {As : list A}
              {a : A}
-             (l : list (f a))
              (l' : list (ilist f As))
-  : list (ilist f (a :: As)) :=
-    (flat_map (fun l' => map (fun fa => icons _ fa l') l) l').
+             (c : ilist f As -> Comp (list (f a)))
+  : Comp (list (ilist f (a :: As))) :=
+    flatten_CompList (map (fun l' => l <- c l'; ret (map (fun fa => icons _ fa l') l)) l').
 
   Definition Build_single_Tuple_list
              {heading}
              (l : list (@Tuple heading))
   : list (ilist (@Tuple) [heading])
     := map (fun a => icons _ a (inil _)) l.
+
+  Lemma filter_and_join_ilist_tail
+        {A}
+        {a}
+        {As}
+        (f' : A -> Type)
+  : forall
+      (f : (ilist f' As) -> bool)
+      (s1 : list (ilist f' As))
+      (s2 : ilist f' As -> Comp (list (f' a)))
+      filter_rest,
+      (forall a, List.In a s1 -> exists v, computes_to (s2 a) v)
+      -> refineEquiv (l <- (Join_Lists s1 s2);
+                   ret (filter (fun x : ilist f' (a :: As) => f (ilist_tl x) && filter_rest x) l))
+                     (l <- Join_Lists (filter f s1) s2;
+                      ret (filter filter_rest l)).
+  Proof.
+    split; induction s1; unfold Join_Lists in *; simpl in *; intros; eauto.
+    - simplify with monad laws; simpl; intros v Comp_v;
+      inversion_by computes_to_inv; subst; repeat econstructor.
+    - simplify with monad laws; intros v.
+      case_eq (f a0); simpl; intros a0_eq Comp_v.
+      + inversion_by computes_to_inv; subst; econstructor; eauto.
+        pose (IHs1 (fun a In_a => H _ (or_intror In_a)) _ (BindComputes _ H3 (ReturnComputes _))); inversion_by computes_to_inv; subst.
+        econstructor; eauto.
+        repeat rewrite filter_app, filter_map; rewrite H4; simpl.
+        rewrite a0_eq, filter_and, filter_true; eauto.
+      + pose (IHs1 (fun a In_a => H _ (or_intror In_a)) _ Comp_v); inversion_by computes_to_inv; subst.
+        destruct (H a0); eauto.
+        repeat (econstructor; eauto).
+        rewrite filter_app, filter_map; simpl; intros;
+        rewrite a0_eq, filter_false; constructor.
+    - intros v Comp_v; inversion_by computes_to_inv; subst; eauto.
+    - intros v Comp_v; inversion_by computes_to_inv; subst.
+      pose proof (IHs1 (fun a In_a => H _ (or_intror In_a)) _
+                 (BindComputes _ H3 (ReturnComputes _))).
+      inversion_by computes_to_inv.
+      case_eq (f a0); intros a0_eq; simpl.
+      + repeat (econstructor; eauto).
+        repeat rewrite filter_app, filter_map; rewrite H4, filter_and; simpl.
+        rewrite a0_eq, filter_and, filter_true; eauto.
+      + repeat (econstructor; eauto).
+        repeat rewrite filter_app, filter_map, filter_and; rewrite H4; simpl.
+        rewrite a0_eq, filter_false; eauto.
+  Qed.
+
+  Corollary filter_join_ilist_tail
+        {A}
+        {a}
+        {As}
+        (f' : A -> Type)
+  : forall
+      (f : (ilist f' As) -> bool)
+      (s1 : list (ilist f' As))
+      (s2 : ilist f' As -> Comp (list (f' a))),
+      (forall a, List.In a s1 -> exists v, computes_to (s2 a) v)
+      -> refineEquiv (l <- (Join_Lists s1 s2);
+                   ret (filter (fun x : ilist f' (a :: As) => f (ilist_tl x)) l))
+                     (Join_Lists (filter f s1) s2).
+  Proof.
+    intros; pose proof (filter_and_join_ilist_tail f s1 s2 (fun _ => true)).
+    setoid_rewrite filter_and in H0; setoid_rewrite filter_true in H0.
+    setoid_rewrite H0; eauto; setoid_rewrite refineEquiv_unit_bind; reflexivity.
+  Qed.
 
   Lemma refine_Query_In_Enumerate
         (ResultT : Type) :
@@ -115,7 +181,7 @@ Section BagsQueryStructureRefinements.
     UnIndexedEnsembleListEquivalence in *.
     intuition; destruct_ex; intuition; subst.
     econstructor; eauto.
-    econstructor; rewrite (H idx); eauto.
+    econstructor; rewrite ((proj1 H) idx); eauto.
     unfold Build_single_Tuple_list in *; rewrite map_map.
     repeat rewrite map_map in H2; simpl in *; eauto.
   Qed.
@@ -158,7 +224,6 @@ Section BagsQueryStructureRefinements.
       repeat econstructor; eauto.
   Qed.
 
-
   Lemma refine_Join_Query_In_Enumerate'
         headings
         (ResultT : Type) :
@@ -171,18 +236,19 @@ Section BagsQueryStructureRefinements.
              l,
         refine (List_Query_In l (fun tup : ilist (@Tuple) headings =>
                                    UnConstrQuery_In r_o idx (resultComp tup)))
-               (l' <- CallBagMethod idx {|bindex := "Enumerate" |} r_n ();
-                List_Query_In (Join_Lists (snd l') l)
-                              (fun tup_pair => (resultComp (ilist_tl tup_pair) (ilist_hd tup_pair)))).
+               (l' <- (Join_Lists l (fun _ => l <- (CallBagMethod idx {|bindex := "Enumerate" |} r_n ());
+                                     ret (snd l)));
+                List_Query_In l' (fun tup_pair => (resultComp (ilist_tl tup_pair) (ilist_hd tup_pair)))).
   Proof.
     intros.
-    unfold List_Query_In; induction l; simpl.
+    unfold List_Query_In; induction l; unfold Join_Lists; simpl.
     - intros v Comp_v; inversion_by computes_to_inv; subst; eauto.
     - setoid_rewrite IHl; rewrite refine_Query_In_Enumerate; eauto.
       unfold List_Query_In.
       setoid_rewrite refineEquiv_bind_bind at 1.
       setoid_rewrite refineEquiv_bind_bind at 2.
       intros v Comp_v; inversion_by computes_to_inv.
+      subst.
       rewrite map_app, map_map in H2; simpl in *.
       econstructor; eauto.
       apply flatten_CompList_app_inv in H2; destruct_ex; intuition.
@@ -202,9 +268,10 @@ Section BagsQueryStructureRefinements.
                               (fun tup =>
                                  UnConstrQuery_In r_o idx' (resultComp (ilist_hd tup))))
                (l <- CallBagMethod idx {|bindex := "Enumerate" |} r_n ();
-                l' <- CallBagMethod idx' {|bindex := "Enumerate" |} r_n ();
-                List_Query_In (Join_Lists (snd l') (Build_single_Tuple_list (snd l)))
-                              (fun tup_pair => (resultComp (ilist_hd (ilist_tl tup_pair)) (ilist_hd tup_pair)))).
+                l' <- (Join_Lists (Build_single_Tuple_list (snd l))
+                                  (fun _ => l <- (CallBagMethod idx' {|bindex := "Enumerate" |} r_n ());
+                                   ret (snd l)));
+                List_Query_In l' (fun tup_pair => (resultComp (ilist_hd (ilist_tl tup_pair)) (ilist_hd tup_pair)))).
   Proof.
     intros.
     f_equiv; simpl; intro.
@@ -238,8 +305,8 @@ Section BagsQueryStructureRefinements.
              (resultComp : Tuple -> Comp (list ResultT)),
         ExtensionalEq filter_dec
                       (BagMatchSearchTerm (ith_Bounded relName BagIndexKeys idx) search_pattern)
-        -> refine (For (l <- CallBagMethod idx {|bindex := "Enumerate" |} r_n ();
-                        List_Query_In (filter filter_dec (snd l)) resultComp))
+        -> refine (l <- CallBagMethod idx {|bindex := "Enumerate" |} r_n ();
+                   List_Query_In (filter filter_dec (snd l)) resultComp)
                   (l <- CallBagMethod idx {|bindex := "Find" |} r_n search_pattern;
                    List_Query_In (snd l) resultComp).
   Proof.
@@ -250,7 +317,7 @@ Section BagsQueryStructureRefinements.
       setoid_rewrite refineEquiv_bind_unit; simpl; f_equiv; intro.
     unfold List_Query_In.
     rewrite (filter_by_equiv _ _ H0).
-    intros v Comp_v; econstructor; eauto.
+    reflexivity.
   Qed.
 
   Instance DecideableEnsemblePair_tail
@@ -279,58 +346,69 @@ Section BagsQueryStructureRefinements.
     intro; apply (dec_decides_P (DecideableEnsemble := P_dec) (ilist_hd a0)).
   Defined.
 
-  Lemma filter_join_ilist_hd
+  Lemma Join_Lists_nil
+        {A}
+        {a}
+        {As}
+        (f' : A -> Type)
+  : forall (s2 : _ -> Comp (list (f' a))),
+      refineEquiv (Join_Lists (As := As) (a := a) [] s2) (ret []).
+  Proof.
+    unfold Join_Lists; simpl; try reflexivity.
+  Qed.
+
+  Lemma filter_and_join_ilist_hd
         {A}
         {a}
         {As}
         (f' : A -> Type)
   : forall
       (f : f' a -> bool)
-      (s2 : list (ilist f' As))
-      (s1 : list (f' a)),
-      filter (fun x : ilist f' (a :: As) => f (ilist_hd x))
-             (Join_Lists s1 s2) =
-      Join_Lists (filter f s1) s2.
+      (s1 : list (ilist f' As))
+      (s2 : _ -> Comp (list (f' a)))
+      filter_rest ,
+      refineEquiv (l <- (Join_Lists s1 s2);
+                   ret (filter (fun x : ilist f' (a :: As) => f (ilist_hd x) && filter_rest x) l))
+                  (l <- Join_Lists s1 (fun a => l <- s2 a; ret (filter f l));
+                   ret (filter filter_rest l)).
   Proof.
-    induction s2; simpl; intros; eauto.
-    rewrite filter_app, IHs2; f_equal.
-    induction s1; simpl; eauto.
-    rewrite IHs1; destruct (f a1); simpl; eauto.
+    split; induction s1; unfold Join_Lists in *; simpl in *; intros; eauto.
+    - simplify with monad laws; rewrite refineEquiv_bind_unit;
+      reflexivity.
+    - simplify with monad laws; intros v Comp_v;
+      inversion_by computes_to_inv; subst; econstructor; eauto.
+      pose (IHs1 _ (BindComputes _ H2 (ReturnComputes _))).
+      inversion_by computes_to_inv; subst.
+      repeat (econstructor; eauto).
+      repeat rewrite filter_app, filter_map; simpl; eauto.
+      rewrite <- filter_and, H3; eauto.
+    - intros v Comp_v; inversion_by computes_to_inv; subst; eauto.
+    - simplify with monad laws; intros v Comp_v;
+      inversion_by computes_to_inv; subst; econstructor; eauto.
+      pose proof (IHs1 _ (BindComputes _ H2 (ReturnComputes _))).
+      inversion_by computes_to_inv; subst.
+      repeat (econstructor; eauto).
+      rewrite filter_app, filter_map; simpl; eauto.
+      repeat rewrite filter_app, filter_map; simpl; eauto.
+      rewrite <- filter_and, H3; eauto.
   Qed.
 
-  Lemma Join_Lists_nil
-        {A}
-        {a}
-        {As}
-        (f' : A -> Type)
-  : forall (s2 : list (ilist f' As)),
-      Join_Lists (a := a) [] s2 = [].
-  Proof.
-    induction s2; simpl; eauto.
-  Qed.
-
-  Lemma filter_join_ilist_tail
+    Corollary filter_join_ilist_hd
         {A}
         {a}
         {As}
         (f' : A -> Type)
   : forall
-      (f : (ilist f' As) -> bool)
-      (s2 : list (ilist f' As))
-      (s1 : list (f' a)),
-      filter (fun x : ilist f' (a :: As) => f (ilist_tl x))
-                (Join_Lists s1 s2) =
-      Join_Lists s1 (filter f s2).
+      (f : f' a -> bool)
+      (s1 : list (ilist f' As))
+      (s2 : _ -> Comp (list (f' a))),
+      refineEquiv (l <- (Join_Lists s1 s2);
+                   ret (filter (fun x : ilist f' (a :: As) => f (ilist_hd x)) l))
+                  (Join_Lists s1 (fun a => l <- s2 a; ret (filter f l))).
   Proof.
-    induction s2; simpl; intros; eauto.
-    rewrite filter_app, IHs2.
-    rewrite filter_map; simpl.
-    induction s1; simpl.
-    - repeat rewrite Join_Lists_nil; eauto.
-    - destruct (f a0); simpl; eauto.
-      + f_equal; simpl in *.
-        rewrite filter_true; reflexivity.
-      + rewrite filter_false in *; reflexivity.
+    intros; pose proof (filter_and_join_ilist_hd f s1 s2 (fun _ => true)).
+    setoid_rewrite filter_and in H; setoid_rewrite filter_true in H.
+    setoid_rewrite H; eauto; setoid_rewrite refineEquiv_unit_bind; reflexivity.
   Qed.
 
   Lemma filter_Build_single_Tuple_list
@@ -343,7 +421,7 @@ Section BagsQueryStructureRefinements.
     destruct (filter_dec a); simpl; congruence.
   Qed.
 
-  Corollary refine_Query_For_In_Find'
+  Corollary refine_Query_For_In_Find_snd'
         (ResultT : Type)
   : forall r_o (r_n : IndexedQueryStructure qs_schema BagIndexKeys),
       DelegateToBag_AbsR r_o r_n
@@ -354,9 +432,9 @@ Section BagsQueryStructureRefinements.
              (resultComp : _ -> Comp (list ResultT)),
         ExtensionalEq filter_dec
                       (BagMatchSearchTerm (ith_Bounded relName BagIndexKeys idx) search_pattern)
-        -> refine (For (l <- CallBagMethod idx {|bindex := "Enumerate" |} r_n ();
+        -> refine (l <- CallBagMethod idx {|bindex := "Enumerate" |} r_n ();
                         List_Query_In (filter (fun tup : ilist (@Tuple) [_] => filter_dec (ilist_hd tup)) (Build_single_Tuple_list (snd l)))
-                                      resultComp))
+                                      resultComp)
                   (l <- CallBagMethod idx {|bindex := "Find" |} r_n search_pattern;
                    List_Query_In (Build_single_Tuple_list (snd l)) resultComp).
   Proof.
@@ -369,41 +447,126 @@ Section BagsQueryStructureRefinements.
       setoid_rewrite refineEquiv_bind_unit; simpl; f_equiv; intro.
     unfold List_Query_In.
     rewrite (filter_by_equiv _ _ H0).
-    intros v Comp_v; econstructor; eauto.
+    reflexivity.
   Qed.
 
-  Lemma refine_Join_Lists_Where_snd
-        (ResultT : Type) :
-    forall (r_n : IndexedQueryStructure qs_schema BagIndexKeys) idx idx'
-           (DT : Ensemble Tuple)
-           (DT_Dec : DecideableEnsemble DT)
-           search_pattern
-           (resultComp : Tuple -> Tuple -> Comp (list ResultT)),
-      ExtensionalEq (@dec _ _ DT_Dec)
-                    (BagMatchSearchTerm (ith_Bounded relName BagIndexKeys idx') search_pattern)
-      -> refine (For (l <- CallBagMethod idx {| bindex := "Enumerate" |} r_n ();
-                      l' <- CallBagMethod idx' {| bindex := "Enumerate" |} r_n ();
-                      List_Query_In (Join_Lists (snd l') (Build_single_Tuple_list (snd l)))
-                                    (fun tup_pair =>
-                                       Where (DT (ilist_hd tup_pair))
-                                             (resultComp (ilist_hd tup_pair) (ilist_hd (ilist_tl tup_pair))))))
+    Corollary refine_Query_For_In_Find_single
+              (ResultT : Type)
+    : forall r_o (r_n : IndexedQueryStructure qs_schema BagIndexKeys),
+        DelegateToBag_AbsR r_o r_n ->
+      forall (idx : @BoundedString (map relName (qschemaSchemas qs_schema)))
+             search_pattern
+             (resultComp : _ -> Comp (list ResultT))
+             filter_rest,
+        refine (l <- CallBagMethod idx {|bindex := "Enumerate" |} r_n ();
+                   List_Query_In (filter (fun a : ilist (@Tuple) [_] => BagMatchSearchTerm _ search_pattern (ilist_hd a) && filter_rest a) (Build_single_Tuple_list (snd l)))
+                                 resultComp)
+                  (l <- CallBagMethod idx {|bindex := "Find" |} r_n search_pattern;
+                   List_Query_In (filter filter_rest (Build_single_Tuple_list (snd l))) resultComp).
+    Proof.
+      unfold CallBagMethod; simpl; intros.
+      simplify with monad laws.
+      setoid_rewrite refineEquiv_bind_bind;
+        setoid_rewrite refineEquiv_bind_unit; simpl;
+        f_equiv; intro.
+      setoid_rewrite <- filter_Build_single_Tuple_list; rewrite filter_and;
+      f_equiv.
+    Qed.
 
-                (For (l <- CallBagMethod idx {| bindex := "Enumerate" |} r_n ();
-                      l' <- CallBagMethod idx' {| bindex := "Find" |} r_n search_pattern;
-                      List_Query_In
-                        (Join_Lists (snd l') (Build_single_Tuple_list (snd l)))
-                                    (fun tup_pair =>
-                                       (resultComp (ilist_hd tup_pair) (ilist_hd (ilist_tl tup_pair)))))).
+  Add Parametric Morphism
+      (A : Type)
+      (f : A -> Type)
+      (As : list A)
+      (a : A)
+      (l' : list (ilist f As))
+      : (@Join_Lists A f As a l')
+      with signature
+      (pointwise_relation _ refineEquiv) ==> refineEquiv
+        as refineEquiv_Join_Lists.
   Proof.
-    intros; repeat f_equiv; simpl; intro.
-    unfold CallBagMethod; simpl.
-    repeat setoid_rewrite refineEquiv_bind_bind;
-      repeat setoid_rewrite refineEquiv_bind_unit;
-      f_equiv; unfold pointwise_relation; intro; simpl.
-    setoid_rewrite <- (filter_by_equiv _ _ H).
-    setoid_rewrite refine_List_Query_In_Where; simpl.
-    instantiate (1 := _); simpl.
-    rewrite filter_join_ilist_hd; f_equiv.
+    unfold pointwise_relation; simpl; intros.
+    induction l'; unfold Join_Lists; simpl.
+    - reflexivity.
+    - rewrite H; setoid_rewrite IHl'; reflexivity.
+  Qed.
+
+  Lemma Join_Lists_apply_f
+        {A B C : Type}
+        {f : A -> Type}
+  : forall (As : list A)
+           (a : A)
+           (l : list (ilist f As))
+           (c : ilist f As -> Comp (list (f a)))
+           (c' : B -> Comp C) (f' : list (ilist f (a :: As)) -> B),
+      refineEquiv (l' <- Join_Lists l c;
+                   c' (f' l'))
+                  (l' <- (l' <- Join_Lists l c; ret (f' l'));
+                   c' l').
+  Proof.
+    split; rewrite refineEquiv_bind_bind;
+    setoid_rewrite refineEquiv_bind_unit;
+    intros v Comp_v; inversion_by computes_to_inv;
+    try econstructor; eauto.
+  Qed.
+
+  Lemma refine_Join_Lists_filter_search_term_snd
+        (ResultT : Type) :
+    forall (r_n : IndexedQueryStructure qs_schema BagIndexKeys)
+           headings
+           idx'
+           search_pattern
+           (resultComp : ilist (@Tuple) (_ :: headings) -> Comp (list ResultT))
+           filter_rest
+           cl,
+      refine (l' <- (Join_Lists cl
+                          (fun _ => l <- CallBagMethod idx' {| bindex := "Enumerate" |} r_n ();
+                           ret (snd l)));
+                 List_Query_In (filter (fun a : ilist (@Tuple) (_ :: headings) => BagMatchSearchTerm _ search_pattern (ilist_hd a) && filter_rest a) l')
+                               resultComp)
+                (l' <- (Join_Lists cl
+                                   (fun _ => l <- CallBagMethod idx' {| bindex := "Find" |} r_n search_pattern;
+                                             ret (snd l)));
+                      List_Query_In (filter filter_rest l') resultComp).
+  Proof.
+    intros; unfold CallBagMethod; simpl.
+    repeat setoid_rewrite (refineEquiv_bind_bind);
+      repeat setoid_rewrite refineEquiv_bind_unit; simpl.
+    setoid_rewrite Join_Lists_apply_f
+    with (c' := fun l =>  List_Query_In l _).
+    setoid_rewrite (refineEquiv_bind_bind) at 2;
+      repeat setoid_rewrite refineEquiv_bind_unit; simpl.
+    setoid_rewrite refineEquiv_unit_bind; simpl.
+    rewrite (filter_and_join_ilist_hd
+               (As := headings) (f' := @Tuple)
+               (BagMatchSearchTerm _ search_pattern)
+               cl
+               (fun _ : ilist (@Tuple) headings =>
+                  {l : list Tuple |
+                   EnsembleIndexedListEquivalence (GetIndexedRelation r_n idx') l})) by eauto.
+    simplify with monad laws; f_equiv.
+  Qed.
+
+  Corollary refine_Join_Lists_filter_search_term_snd'
+        (ResultT : Type) :
+    forall (r_n : IndexedQueryStructure qs_schema BagIndexKeys)
+           idx idx'
+           search_pattern
+           (resultComp : ilist (@Tuple) [_; _] -> Comp (list ResultT))
+           filter_rest,
+      refine (cl <- CallBagMethod idx {| bindex := "Enumerate" |} r_n ();
+              l' <- (Join_Lists (Build_single_Tuple_list (snd cl))
+                          (fun _ => l <- CallBagMethod idx' {| bindex := "Enumerate" |} r_n ();
+                           ret (snd l)));
+                 List_Query_In (filter (fun a : ilist (@Tuple) [_ ; _] => BagMatchSearchTerm _ search_pattern (ilist_hd a) && filter_rest a) l')
+                               resultComp)
+             (cl <- CallBagMethod idx {| bindex := "Enumerate" |} r_n ();
+              l' <- (Join_Lists (Build_single_Tuple_list (snd cl))
+                                   (fun _ => l <- CallBagMethod idx' {| bindex := "Find" |} r_n search_pattern;
+                                             ret (snd l)));
+                      List_Query_In (filter filter_rest l') resultComp).
+  Proof.
+    intros; f_equiv; intro.
+    apply refine_Join_Lists_filter_search_term_snd.
   Qed.
 
   Lemma refine_List_Query_In_Return
@@ -417,6 +580,167 @@ Section BagsQueryStructureRefinements.
     - unfold Query_Return; simplify with monad laws;
       setoid_rewrite IHl; simplify with monad laws;
       reflexivity.
+  Qed.
+
+  Lemma filter_and_join_ilist_hd_dep
+        {A}
+        {a}
+        {As}
+        (f' : A -> Type)
+  : forall
+      (f : ilist f' As -> f' a -> bool)
+      (s1 : list (ilist f' As))
+      (s2 : _ -> Comp (list (f' a)))
+      filter_rest,
+      refineEquiv (l <- (Join_Lists s1 s2);
+                   ret (filter (fun x : ilist f' (a :: As) => f (ilist_tl x) (ilist_hd x) && filter_rest x) l))
+                  (l <- Join_Lists s1 (fun a => l <- s2 a; ret (filter (f a) l));
+                   ret (filter filter_rest l)).
+  Proof.
+    split; induction s1; unfold Join_Lists in *; simpl in *; intros; eauto.
+    - simplify with monad laws; rewrite refineEquiv_bind_unit; reflexivity.
+    - simplify with monad laws; intros v Comp_v;
+      inversion_by computes_to_inv; subst; econstructor; eauto.
+      pose (IHs1 _ (BindComputes _ H2 (ReturnComputes _))).
+      inversion_by computes_to_inv; subst.
+      repeat (econstructor; eauto).
+      repeat rewrite filter_app, filter_map; simpl; eauto.
+      rewrite <- filter_and, H3; eauto.
+    - intros v Comp_v; inversion_by computes_to_inv; subst; eauto.
+    - simplify with monad laws; intros v Comp_v;
+      inversion_by computes_to_inv; subst; econstructor; eauto.
+      pose proof (IHs1 _ (BindComputes _ H2 (ReturnComputes _))).
+      inversion_by computes_to_inv; subst.
+      repeat (econstructor; eauto).
+      rewrite filter_app, filter_map; simpl; eauto.
+      repeat rewrite filter_app, filter_map; simpl; eauto.
+      rewrite <- filter_and, H3; eauto.
+  Qed.
+
+    Lemma refine_Join_Lists_filter_search_term_snd_dep
+        (ResultT : Type) :
+    forall (r_n : IndexedQueryStructure qs_schema BagIndexKeys)
+           headings
+           idx'
+           (search_pattern : _ -> _)
+           (resultComp : ilist (@Tuple) (_ :: headings) -> Comp (list ResultT))
+           filter_rest
+           (cl : list (ilist (@Tuple) headings)),
+      refine (l' <- (Join_Lists cl
+                          (fun _ => l <- CallBagMethod idx' {| bindex := "Enumerate" |} r_n ();
+                           ret (snd l)));
+                 List_Query_In (filter (fun a : ilist (@Tuple) (_ :: headings) => BagMatchSearchTerm _ (search_pattern (ilist_tl a)) (ilist_hd a) && filter_rest a) l')
+                               resultComp)
+                (l' <- (Join_Lists cl
+                                   (fun tup => l <- CallBagMethod idx' {| bindex := "Find" |} r_n (search_pattern tup);
+                                             ret (snd l)));
+                      List_Query_In (filter filter_rest l') resultComp).
+  Proof.
+    intros; unfold CallBagMethod; simpl.
+    repeat setoid_rewrite (refineEquiv_bind_bind);
+      repeat setoid_rewrite refineEquiv_bind_unit; simpl.
+    setoid_rewrite Join_Lists_apply_f
+    with (c' := fun l =>  List_Query_In l _).
+    setoid_rewrite (refineEquiv_bind_bind) at 2;
+      repeat setoid_rewrite refineEquiv_bind_unit; simpl.
+    setoid_rewrite refineEquiv_unit_bind; simpl.
+    rewrite filter_and_join_ilist_hd_dep with
+    (f := fun tup =>  (BagMatchSearchTerm
+                (ith_Bounded' relName (qschemaSchemas qs_schema)
+                   (nth_error_map relName (ibound idx')
+                      (qschemaSchemas qs_schema) (boundi idx'))
+                   (ith_error BagIndexKeys (ibound idx')))
+                (search_pattern tup))).
+    simplify with monad laws; f_equiv.
+  Qed.
+
+  Lemma realizeable_Enumerate
+  : forall
+      (r_n : IndexedQueryStructure qs_schema BagIndexKeys)
+      (r_o : UnConstrQueryStructure qs_schema)
+      idx,
+      DelegateToBag_AbsR r_o r_n ->
+      exists v : list Tuple,
+        (l <- CallBagMethod idx {| bindex := "Enumerate"|} r_n ();
+         ret (snd l)) ↝ v.
+  Proof.
+    intros; destruct H as [r_o_eq H]; destruct (H idx) as [l l_eqv].
+    rewrite (r_o_eq idx) in l_eqv.
+    eexists l; unfold CallBagMethod; simpl; eauto.
+  Qed.
+
+  Lemma realizeable_Find
+  : forall
+      (r_n : IndexedQueryStructure qs_schema BagIndexKeys)
+      (r_o : UnConstrQueryStructure qs_schema)
+      idx st,
+      DelegateToBag_AbsR r_o r_n ->
+      exists v : list Tuple,
+        (l <- CallBagMethod idx {| bindex := "Find"|} r_n st;
+         ret (snd l)) ↝ v.
+  Proof.
+    intros; destruct H as [r_o_eq H]; destruct (H idx) as [l l_eqv].
+    rewrite (r_o_eq idx) in l_eqv.
+    eexists (filter _ l); unfold CallBagMethod; simpl; eauto.
+    econstructor; eauto.
+    simpl; eauto.
+  Qed.
+
+  Corollary refine_Join_Lists_filter_search_term_snd_dep'
+        (ResultT : Type) :
+    forall (r_n : IndexedQueryStructure qs_schema BagIndexKeys)
+           idx idx'
+           (search_pattern : _ -> _)
+           (resultComp : ilist (@Tuple) [_; _] -> Comp (list ResultT))
+           filter_rest,
+      refine (cl <- CallBagMethod idx {| bindex := "Enumerate" |} r_n ();
+              l' <- (Join_Lists (Build_single_Tuple_list (snd cl))
+                          (fun _ => l <- CallBagMethod idx' {| bindex := "Enumerate" |} r_n ();
+                           ret (snd l)));
+                 List_Query_In (filter (fun a : ilist (@Tuple) [_ ; _] => BagMatchSearchTerm _ (search_pattern (ilist_tl a)) (ilist_hd a) && filter_rest a) l')
+                               resultComp)
+             (cl <- CallBagMethod idx {| bindex := "Enumerate" |} r_n ();
+              l' <- (Join_Lists (Build_single_Tuple_list (snd cl))
+                                   (fun tup => l <- CallBagMethod idx' {| bindex := "Find" |} r_n (search_pattern tup);
+                                             ret (snd l)));
+                      List_Query_In (filter filter_rest l') resultComp).
+  Proof.
+    intros; f_equiv; intro;
+    apply refine_Join_Lists_filter_search_term_snd_dep.
+  Qed.
+
+  Lemma refine_Join_Lists_filter_search_term_fst
+        (ResultT : Type) :
+    forall (r_n : IndexedQueryStructure qs_schema BagIndexKeys)
+           idx
+           heading
+           cl
+           (search_pattern : _)
+           (resultComp : ilist (@Tuple) [heading ; _] -> Comp (list ResultT))
+           (cl_realizable : forall a, exists v, computes_to (cl a) v)
+           filter_rest,
+      refine (l <- CallBagMethod idx {| bindex := "Enumerate" |} r_n ();
+              l' <- Join_Lists (Build_single_Tuple_list (snd l)) cl;
+              List_Query_In (filter (fun a : ilist (@Tuple) [_ ; _] => (BagMatchSearchTerm _ search_pattern (ilist_hd (ilist_tl a)) && filter_rest a)) l')
+                            resultComp)
+             (l <- CallBagMethod idx {| bindex := "Find" |} r_n search_pattern;
+              l' <- Join_Lists (Build_single_Tuple_list (snd l)) cl;
+              List_Query_In (filter filter_rest l') resultComp).
+  Proof.
+    intros; unfold CallBagMethod; simpl.
+    repeat setoid_rewrite (refineEquiv_bind_bind);
+      repeat setoid_rewrite refineEquiv_bind_unit; simpl.
+    f_equiv; unfold pointwise_relation; intros.
+    setoid_rewrite Join_Lists_apply_f
+    with (c' := fun l =>  List_Query_In l resultComp).
+    setoid_rewrite (refineEquiv_bind_bind) at 2;
+      repeat setoid_rewrite refineEquiv_bind_unit; simpl.
+    rewrite (filter_and_join_ilist_tail
+              (fun a0 : ilist (@Tuple) [_] =>_ (ilist_hd a0))
+              (Build_single_Tuple_list a)) by eauto.
+    simplify with monad laws; f_equiv.
+    unfold Build_single_Tuple_list; simpl;
+    repeat rewrite filter_map; f_equiv.
   Qed.
 
   Require Import ADTSynthesis.QueryStructure.Implementation.Operations.General.DeleteRefinements.
@@ -440,7 +764,7 @@ Section BagsQueryStructureRefinements.
     setoid_rewrite refine_List_Query_In_Where.
     instantiate (1 := _).
     simpl in *.
-    setoid_rewrite (refine_Query_For_In_Find' H _ H0).
+    setoid_rewrite (refine_Query_For_In_Find_snd' H _ H0).
     setoid_rewrite refine_List_Query_In_Return.
     unfold Build_single_Tuple_list; setoid_rewrite map_map; simpl.
     setoid_rewrite map_id.
@@ -448,7 +772,43 @@ Section BagsQueryStructureRefinements.
     setoid_rewrite refineEquiv_bind_bind;
     setoid_rewrite refineEquiv_bind_unit; simpl;
     f_equiv; intro.
+    refine pick val _; eauto.
+    reflexivity.
   Qed.
+
+  Lemma NoDup_filter {A} :
+    forall (f : A -> bool)
+           (l : list A),
+      NoDup l
+      -> NoDup (filter f l).
+  Proof.
+    induction l; simpl.
+    - constructor.
+    - case_eq (f a); simpl; intros.
+      + inversion H0; constructor; eauto.
+        subst; unfold not; intros H1;
+        apply filter_In in H1; intuition.
+      + inversion H0; eauto.
+  Qed.
+
+  Lemma NoDup_filter_map {A} :
+    forall (f : A -> bool)
+           (l : list _),
+      NoDup (map elementIndex l)
+      -> NoDup
+           (map elementIndex
+                (filter (fun a => f (indexedElement a)) l)) .
+  Proof.
+    induction l; simpl.
+    - constructor.
+    - case_eq (f (indexedElement a)); simpl; intros; inversion H0; subst; eauto.
+      constructor; eauto.
+      unfold not; intros; apply H3.
+      revert H1; clear; induction l; simpl.
+      + eauto.
+      + case_eq (f (indexedElement a0)); simpl; intros; intuition.
+  Qed.
+
 
   Lemma refine_BagADT_QSDelete_snd :
     forall r_o (r_n : IndexedQueryStructure qs_schema BagIndexKeys),
@@ -472,21 +832,43 @@ Section BagsQueryStructureRefinements.
     constructor; inversion_by computes_to_inv.
     unfold CallBagMethod in *; simpl in *; inversion_by computes_to_inv; subst.
     simpl.
-    unfold DelegateToBag_AbsR; intros.
-    destruct (BoundedString_eq_dec idx idx0); subst.
-    - unfold GetUnConstrRelation, UpdateUnConstrRelation;
-      rewrite ith_replace_BoundIndex_eq.
-      unfold GetIndexedRelation, UpdateIndexedRelation;
-      rewrite i2th_replace_BoundIndex_eq.
-      f_equal; eauto.
-      apply Extensionality_Ensembles; unfold Same_set, Included, In;
-      intuition; rewrite <- H0 in *;
-      eapply dec_decides_P; eauto.
-    - unfold GetUnConstrRelation, UpdateUnConstrRelation;
-      rewrite ith_replace_BoundIndex_neq by eauto using string_dec.
-      unfold GetIndexedRelation, UpdateIndexedRelation;
-      rewrite i2th_replace_BoundIndex_neq by eauto using string_dec.
-      apply H.
+    unfold DelegateToBag_AbsR; split; intros.
+    - destruct (BoundedString_eq_dec idx idx0); subst.
+      + unfold GetUnConstrRelation, UpdateUnConstrRelation;
+        rewrite ith_replace_BoundIndex_eq.
+        unfold GetIndexedRelation, UpdateIndexedRelation;
+          rewrite i2th_replace_BoundIndex_eq.
+        f_equal; eauto.
+        * eapply H.
+        * apply Extensionality_Ensembles; unfold Same_set, Included, In;
+          intuition; rewrite <- H0 in *;
+          eapply dec_decides_P; eauto.
+      + unfold GetUnConstrRelation, UpdateUnConstrRelation;
+        rewrite ith_replace_BoundIndex_neq by eauto using string_dec.
+        unfold GetIndexedRelation, UpdateIndexedRelation;
+          rewrite i2th_replace_BoundIndex_neq by eauto using string_dec.
+        apply H.
+    - destruct H.
+      destruct (BoundedString_eq_dec idx idx0); subst.
+      + rewrite get_update_unconstr_eq.
+        destruct (H1 idx0) as [l [[bnd fresh_bnd] [l' [l'_eq [l_eqv NoDup_l']]]]].
+        exists (filter (fun a => negb (dec a)) l); split.
+        * exists bnd; unfold EnsembleDelete, UnConstrFreshIdx; intros.
+          inversion H3; subst; eauto.
+        * unfold UnIndexedEnsembleListEquivalence;
+          exists (filter (fun a => negb (dec (indexedElement a))) l'); split; eauto.
+          rewrite <- l'_eq; rewrite filter_map; reflexivity.
+          intuition.
+          apply filter_In; split.
+          eapply l_eqv; inversion H3; eauto.
+          inversion H3; subst; rewrite (proj2 (Decides_false _ _)); eauto.
+          rewrite filter_In in H3; intuition; constructor;
+          [ apply l_eqv; eauto
+            | case_eq (dec (indexedElement x)); intros H'; rewrite H' in H5;
+              try discriminate;
+              eapply Decides_false in H'; eauto ].
+          eapply NoDup_filter_map with (f := fun a => negb (dec a)); eauto.
+      + rewrite get_update_unconstr_neq; eauto.
   Qed.
 
 End BagsQueryStructureRefinements.
